more work

Common/Rel.lean
@@ -3,7 +3,9 @@ variable {α : Sort u} (r : α → α → Prop)
 class Reflexive : Prop where
   refl : r x x
 
-theorem Reflexive.ofEq {r : α → α → Prop} [Reflexive r] {x y} (h : x = y) : r x y := h ▸ refl
+variable {r} in
+theorem Reflexive.ofEq [Reflexive r] {x y} (h : x = y) : r x y :=
+  h ▸ refl
 
 class Symmetric : Prop where
   symm : r x y → r y x
@@ -11,67 +13,325 @@ class Symmetric : Prop where
 class Transitive : Prop where
   trans : r x y → r y z → r x z
 
-class abbrev Equivalence' : Prop := Reflexive r, Symmetric r, Transitive r
+inductive ReflexiveClosure : α → α → Prop
+  | base : r x y → ReflexiveClosure x y
+  | refl : ReflexiveClosure x x
 
-inductive ReflexiveTransitiveClosure : α → α → Prop
-  | base : r x y → ReflexiveTransitiveClosure x y
-  | refl : ReflexiveTransitiveClosure x x
-  | trans : ReflexiveTransitiveClosure x y → ReflexiveTransitiveClosure y z → ReflexiveTransitiveClosure x z
+namespace ReflexiveClosure
 
-instance ReflexiveTransitiveClosure.instReflexive : Reflexive (ReflexiveTransitiveClosure r) := ⟨@refl α r⟩
-instance ReflexiveTransitiveClosure.instTransitive : Transitive (ReflexiveTransitiveClosure r) := ⟨@trans α r⟩
+instance instReflexive : Reflexive (ReflexiveClosure r) := ⟨@refl α r⟩
 
 section rec
 
-variable {r} {motive : ∀ x y, ReflexiveTransitiveClosure r x y → Prop}
+variable {r} {motive : ∀ x y, ReflexiveClosure r x y → Prop}
   (base : ∀ {x y} h, motive x y (base h))
   (refl : ∀ {x}, motive x x refl)
 
-def ReflexiveTransitiveClosure.recl
-  (trans : ∀ {x y z} h₁ h₂, motive x y h₁ → motive x z (trans h₁ (.base h₂)))
+theorem rec' {x} : ∀ {y} h, motive x y h :=
+  @rec α r x (motive x) (@base x) refl
+
+end rec
+
+section map
+
+variable {β : Sort v} {r : α → α → Prop} {s : β → β → Prop} {f : α → β}
+
+theorem map [Reflexive s] (h : ∀ {x y}, r x y → s (f x) (f y))
+: ∀ {x y}, ReflexiveClosure r x y → s (f x) (f y) :=
+  @rec' α r _ @h Reflexive.refl
+
+theorem map' (h : ∀ {x y}, r x y → s (f x) (f y))
+: ∀ {x y}, ReflexiveClosure r x y → ReflexiveClosure s (f x) (f y) :=
+  @map α β r _ f _ (base <| h ·)
+
+end map
+
+end ReflexiveClosure
+
+inductive SymmetricClosure : α → α → Prop
+  | base : r x y → SymmetricClosure x y
+  | symm : SymmetricClosure x y → SymmetricClosure y x
+
+namespace SymmetricClosure
+
+instance instSymmetric : Symmetric (SymmetricClosure r) := ⟨@symm α r⟩
+
+section rec
+
+variable {r} {motive : ∀ x y, SymmetricClosure r x y → Prop}
+  (base : ∀ {x y} h, motive x y (base h))
+  (symm : ∀ {x y} h, motive y x (symm (.base h)))
+
+theorem rec' {x y} h : motive x y h :=
+  @rec α r (λ x y h => motive x y h ∧ motive y x (.symm h))
+    (λ h => ⟨base h, symm h⟩)
+    (λ _ ih => ⟨ih.2, ih.1⟩)
+  x y h |>.1
+
+end rec
+
+section map
+
+variable {β : Sort v} {r : α → α → Prop} {s : β → β → Prop} {f : α → β}
+
+theorem map [Symmetric s] (h : ∀ {x y}, r x y → s (f x) (f y))
+: ∀ {x y}, SymmetricClosure r x y → s (f x) (f y) :=
+  @rec α r _ @h λ _ => Symmetric.symm
+
+theorem map' (h : ∀ {x y}, r x y → s (f x) (f y))
+: ∀ {x y}, SymmetricClosure r x y → SymmetricClosure s (f x) (f y) :=
+  @map α β r _ f _ (base <| h ·)
+
+end map
+
+end SymmetricClosure
+
+inductive TransitiveClosure : α → α → Prop
+  | base : r x y → TransitiveClosure x y
+  | trans : TransitiveClosure x y → TransitiveClosure y z → TransitiveClosure x z
+
+namespace TransitiveClosure
+
+instance instTransitive : Transitive (TransitiveClosure r) := ⟨@trans α r⟩
+
+section rec
+
+variable {r} {motive : ∀ x y, TransitiveClosure r x y → Prop}
+  (base : ∀ {x y} h, motive x y (base h))
+
+theorem recl (trans : ∀ {x y z} h₁ h₂, motive x y h₁ → motive x z (trans h₁ (.base h₂)))
 : ∀ {x y} h, motive x y h :=
-  @rec α r motive base refl λ {x y z} h₁ h₂ ih₁ _ =>
+  @rec α r motive @base λ {x y z} h₁ h₂ ih₁ _ =>
     @rec α r (λ y z h₂ => ∀ h₁, motive x y h₁ → motive x z (.trans h₁ h₂))
       (λ h₂ h₁ => trans h₁ h₂)
-      (λ _ ih₁ => ih₁)
       (λ h₂ _ r₁ r₂ h₁ ih₁ => r₁ h₁ ih₁ |> r₂ (.trans h₁ h₂))
     y z h₂ h₁ ih₁
 
-def ReflexiveTransitiveClosure.recr
-  (trans : ∀ {x y z} h₁ h₂, motive y z h₂ → motive x z (trans (.base h₁) h₂))
+theorem recr (trans : ∀ {x y z} h₁ h₂, motive y z h₂ → motive x z (trans (.base h₁) h₂))
 : ∀ {x y} h, motive x y h :=
-  @rec α r motive base refl λ {x y z} h₁ h₂ _ =>
+  @rec α r motive @base λ {x y z} h₁ h₂ _ =>
     @rec α r (λ x y h₁ => ∀ h₂, motive y z h₂ → motive x z (.trans h₁ h₂))
       trans
-      (λ _ ih₂ => ih₂)
       (λ _ h₁ r₁ r₂ h₂ ih₂ => r₁ (.trans h₁ h₂) <| r₂ h₂ ih₂)
     x y h₁ h₂
 
 end rec
 
-def ReflexiveTransitiveClosure.lift {β : Sort v} {r s} {f : α → β} (h : ∀ {x y}, r x y → s (f x) (f y)) :
-  ∀ {x y}, ReflexiveTransitiveClosure r x y → ReflexiveTransitiveClosure s (f x) (f y)
-:=
-  @rec α r _
-    (base <| h ·)
-    refl
-    (λ _ _ => trans)
+section map
 
-inductive EquivalenceClosure : α → α → Prop
-  | base : r x y → EquivalenceClosure x y
-  | refl : EquivalenceClosure x x
-  | symm : EquivalenceClosure x y → EquivalenceClosure y x
-  | trans : EquivalenceClosure x y → EquivalenceClosure y z → EquivalenceClosure x z
+variable {β : Sort v} {r : α → α → Prop} {s : β → β → Prop} {f : α → β}
 
-instance EquivalenceClosure.instReflexive : Reflexive (EquivalenceClosure r) := ⟨@refl α r⟩
-instance EquivalenceClosure.instSymmetric : Symmetric (EquivalenceClosure r) := ⟨@symm α r⟩
-instance EquivalenceClosure.instTransitive : Transitive (EquivalenceClosure r) := ⟨@trans α r⟩
+theorem map [Transitive s] (h : ∀ {x y}, r x y → s (f x) (f y))
+: ∀ {x y}, TransitiveClosure r x y → s (f x) (f y) :=
+  @rec α r _ @h λ _ _ => Transitive.trans
 
-def EquivalenceClosure.lift {β : Sort v} {r s} {f : α → β} (h : ∀ {x y}, r x y → s (f x) (f y)) :
-  ∀ {x y}, EquivalenceClosure r x y → EquivalenceClosure s (f x) (f y)
-:=
-  @rec α r _
-    (base <| h ·)
-    refl
-    (λ _ => symm)
-    (λ _ _ => trans)
+theorem map' (h : ∀ {x y}, r x y → s (f x) (f y))
+: ∀ {x y}, TransitiveClosure r x y → TransitiveClosure s (f x) (f y) :=
+  @map α β r _ f _ (base <| h ·)
+
+end map
+
+end TransitiveClosure
+
+instance SymmetricClosure.instReflexive [Reflexive r] : Reflexive (SymmetricClosure r) where
+  refl := base Reflexive.refl
+
+instance TransitiveClosure.instReflexive [Reflexive r] : Reflexive (TransitiveClosure r) where
+  refl := base Reflexive.refl
+
+instance ReflexiveClosure.instSymmetric [Symmetric r] : Symmetric (ReflexiveClosure r) where
+  symm := @rec' α r _ (λ h => base <| Symmetric.symm h) refl
+
+instance TransitiveClosure.instSymmetric [Symmetric r] : Symmetric (TransitiveClosure r) where
+  symm := @rec α r _ (λ h => base <| Symmetric.symm h) λ _ _ h₁ h₂ => trans h₂ h₁
+
+instance ReflexiveClosure.instTransitive [Transitive r] : Transitive (ReflexiveClosure r) where
+  trans h₁ :=
+    @rec' α r (λ x y _ => ∀ z, ReflexiveClosure r y z → ReflexiveClosure r x z) (λ h₁ z h₂ =>
+      @rec' α r (λ y z _ => ∀ x, r x y → ReflexiveClosure r x z)
+        (λ h₂ _ h₁ => base <| Transitive.trans h₁ h₂)
+        (λ _ => base)
+      _ z h₂ _ h₁
+    ) (λ _ h₂ => h₂) _ _ h₁ _
+
+abbrev ReflexiveTransitiveClosure := ReflexiveClosure (TransitiveClosure r)
+
+namespace ReflexiveTransitiveClosure
+
+variable {r}
+
+theorem base (h : r x y) : ReflexiveTransitiveClosure r x y :=
+  .base (.base h)
+
+theorem refl : ReflexiveTransitiveClosure r x x :=
+  .refl
+
+theorem trans : ReflexiveTransitiveClosure r x y → ReflexiveTransitiveClosure r y z → ReflexiveTransitiveClosure r x z :=
+  Transitive.trans
+
+section rec
+
+variable {motive : ∀ x y, ReflexiveTransitiveClosure r x y → Prop}
+  (base : ∀ {x y} h, motive x y (base h))
+  (refl : ∀ {x}, motive x x refl)
+
+theorem rec (trans : ∀ {x y z} h₁ h₂, motive x y h₁ → motive y z h₂ → motive x z (trans h₁ h₂))
+: ∀ {x y} h, motive x y h :=
+  @ReflexiveClosure.rec' α _ _ (
+    @TransitiveClosure.rec α r _ @base λ h₁ h₂ => @trans _ _ _ (ReflexiveClosure.base h₁) (ReflexiveClosure.base h₂)
+  ) @refl
+
+theorem recl (trans : ∀ {x y z} h₁ h₂, motive x y h₁ → motive x z (trans h₁ (.base h₂)))
+: ∀ {x y} h, motive x y h :=
+  @ReflexiveClosure.rec' α _ _ (
+    @TransitiveClosure.recl α r _ @base λ h₁ => @trans _ _ _ (ReflexiveClosure.base h₁)
+  ) @refl
+
+theorem recr
+  (trans : ∀ {x y z} h₁ h₂, motive y z h₂ → motive x z (trans (.base h₁) h₂))
+: ∀ {x y} h, motive x y h :=
+  @ReflexiveClosure.rec' α _ _ (
+    @TransitiveClosure.recr α r _ @base λ h₁ h₂ => @trans _ _ _ h₁ (ReflexiveClosure.base h₂)
+  ) @refl
+
+end rec
+
+section map
+
+variable {β : Sort v} {r : α → α → Prop} {s : β → β → Prop} {f : α → β}
+
+theorem map [Reflexive s] [Transitive s] (h : ∀ {x y}, r x y → s (f x) (f y))
+: ∀ {x y}, ReflexiveTransitiveClosure r x y → s (f x) (f y) :=
+  @ReflexiveClosure.rec' α _ _ (
+    @TransitiveClosure.rec α r _ @h λ _ _ => Transitive.trans
+  ) Reflexive.refl
+
+theorem map' (h : ∀ {x y}, r x y → s (f x) (f y))
+: ∀ {x y}, ReflexiveTransitiveClosure r x y → ReflexiveTransitiveClosure s (f x) (f y) :=
+  @map α β r _ f _ _ (base <| h ·)
+
+end map
+
+end ReflexiveTransitiveClosure
+
+abbrev EquivalenceClosure := ReflexiveTransitiveClosure (SymmetricClosure r)
+
+namespace EquivalenceClosure
+
+variable {r}
+
+theorem base (h : r x y) : EquivalenceClosure r x y :=
+  .base (.base h)
+
+theorem refl : EquivalenceClosure r x x :=
+  .refl
+
+theorem symm : EquivalenceClosure r x y → EquivalenceClosure r y x :=
+  Symmetric.symm
+
+theorem trans : EquivalenceClosure r x y → EquivalenceClosure r y z → EquivalenceClosure r x z :=
+  .trans
+
+section rec
+
+variable {motive : ∀ x y, EquivalenceClosure r x y → Prop}
+  (base : ∀ {x y} h, motive x y (base h))
+  (refl : ∀ {x}, motive x x refl)
+  (symm : ∀ {x y} h, motive y x (symm (.base h)))
+
+theorem rec (trans : ∀ {x y z} h₁ h₂, motive x y h₁ → motive y z h₂ → motive x z (trans h₁ h₂))
+: ∀ {x y} h, motive x y h :=
+  @ReflexiveClosure.rec' α _ _ (
+    @TransitiveClosure.rec α _ _ (
+      @SymmetricClosure.rec' α r _ @base @symm
+    ) λ h₁ h₂ => @trans _ _ _ (ReflexiveClosure.base h₁) (ReflexiveClosure.base h₂)
+  ) @refl
+
+theorem recl (trans : ∀ {x y z} h₁ h₂, motive x y h₁ → motive x z (trans h₁ (ReflexiveTransitiveClosure.base h₂)))
+: ∀ {x y} h, motive x y h :=
+  @ReflexiveClosure.rec' α _ _ (
+    @TransitiveClosure.recl α _ _ (
+      @SymmetricClosure.rec' α r _ @base @symm
+    ) λ h₁ => @trans _ _ _ (ReflexiveClosure.base h₁)
+  ) @refl
+
+theorem recr
+  (trans : ∀ {x y z} h₁ h₂, motive y z h₂ → motive x z (trans (ReflexiveTransitiveClosure.base h₁) h₂))
+: ∀ {x y} h, motive x y h :=
+  @ReflexiveClosure.rec' α _ _ (
+    @TransitiveClosure.recr α _ _ (
+      @SymmetricClosure.rec' α r _ @base @symm
+    ) λ h₁ h₂ => @trans _ _ _ h₁ (ReflexiveClosure.base h₂)
+  ) @refl
+
+end rec
+
+section map
+
+variable {β : Sort v} {r : α → α → Prop} {s : β → β → Prop} {f : α → β}
+
+theorem map [Reflexive s] [Symmetric s] [Transitive s] (h : ∀ {x y}, r x y → s (f x) (f y))
+: ∀ {x y}, EquivalenceClosure r x y → s (f x) (f y) :=
+  @ReflexiveClosure.rec' α _ _ (
+    @TransitiveClosure.rec α _ _ (
+      @SymmetricClosure.rec α r _ @h λ _ => Symmetric.symm
+    ) λ _ _ => Transitive.trans
+  ) Reflexive.refl
+
+theorem map' (h : ∀ {x y}, r x y → s (f x) (f y))
+: ∀ {x y}, EquivalenceClosure r x y → EquivalenceClosure s (f x) (f y) :=
+  @map α β r _ f _ _ _ (base <| h ·)
+
+end map
+
+end EquivalenceClosure
+
+@[simp]
+theorem ReflexiveClosure_ReflexiveClosure : ReflexiveClosure (ReflexiveClosure r) = ReflexiveClosure r :=
+  funext λ _ => funext λ _ => propext ⟨.map id, .base⟩
+
+@[simp]
+theorem SymmetricClosure_SymmetricClosure : SymmetricClosure (SymmetricClosure r) = SymmetricClosure r :=
+  funext λ _ => funext λ _ => propext ⟨.map id, .base⟩
+
+@[simp]
+theorem TransitiveClosure_TransitiveClosure : TransitiveClosure (TransitiveClosure r) = TransitiveClosure r :=
+  funext λ _ => funext λ _ => propext ⟨.map id, .base⟩
+
+@[simp]
+theorem TransitiveClosure_ReflexiveClosure : TransitiveClosure (ReflexiveClosure r) = ReflexiveTransitiveClosure r :=
+  funext λ _ => funext λ _ => propext ⟨
+    TransitiveClosure.map (f := id) <| ReflexiveClosure.map' .base,
+    ReflexiveTransitiveClosure.map (f := id) λ h => .base <| .base h
+  ⟩
+
+@[simp]
+theorem TransitiveClosure_SymmetricClosure_ReflexiveClosure : TransitiveClosure (SymmetricClosure (ReflexiveClosure r)) = EquivalenceClosure r :=
+  funext λ _ => funext λ _ => propext ⟨
+    TransitiveClosure.map (f := id) <| SymmetricClosure.map <| ReflexiveClosure.map' λ h => .base <| .base h,
+    EquivalenceClosure.map (f := id) λ h => .base <| .base <| .base h
+  ⟩
+
+def Diamond := ∀ {x x₁ x₂}, r x x₁ → r x x₂ → ∃ x', r x₁ x' ∧ r x₂ x'
+
+variable {r} in
+theorem ReflexiveTransitiveClosure.diamond (h : Diamond r) : Diamond (ReflexiveTransitiveClosure r) := λ {x x₁ x₂} h₁ h₂ => by
+  induction h₁ using rec generalizing x₂ with
+  | @base _ x₁ h₁ =>
+    suffices ∃ x', _ ∧ _ from
+      let ⟨x', hx, hx'⟩ := this
+      ⟨x', hx, .base hx'⟩
+    induction h₂ using rec generalizing x₁ with
+    | base h₂ =>
+      let ⟨x₁, hx₁, hx₁'⟩ := h h₁ h₂
+      exact ⟨_, .base hx₁, hx₁'⟩
+    | refl => exact ⟨x₁, .refl, h₁⟩
+    | trans _ _ ih₂ ih₂' =>
+      let ⟨x₁, hx₁, hx₁'⟩ := ih₂ h₁
+      let ⟨x₂, hx₂, hx₂'⟩ := ih₂' hx₁'
+      exact ⟨x₂, .trans hx₁ hx₂, hx₂'⟩
+  | refl => exact ⟨x₂, h₂, refl⟩
+  | trans _ _ ih₁ ih₁' =>
+    let ⟨x₁, hx₁, hx₁'⟩ := ih₁ h₂
+    let ⟨x₂, hx₂, hx₂'⟩ := ih₁' hx₁
+    exact ⟨x₂, hx₂, .trans hx₁' hx₂'⟩
