Lambda.lean
@@ -1,11 +1,5 @@
 import Std
-import Common.Rel
-import Common.Meta
-
-def Fin.zero : Fin (.succ n) := ⟨0, n.zero_lt_succ⟩
-def Fin.last : Fin (.succ n) := ⟨n, n.lt_succ_self⟩
-def Fin.castSucc (i : Fin n) : Fin n.succ := ⟨i, .step i.2⟩
-def Fin.castLe (h : n ≤ m) (i : Fin n) : Fin m := ⟨i, Nat.le_trans i.2 h⟩
+import Common
 
 def Nat.le_add_right_of_le {m n k : Nat} (h : m ≤ n) : m ≤ n + k :=
   Nat.le_trans h (Nat.le_add_right n k)
@@ -13,28 +7,33 @@ def Nat.le_add_right_of_le {m n k : Nat} (h : m ≤ n) : m ≤ n + k :=
 def Nat.le_add_left_of_le {m n k : Nat} (h : m ≤ n) : m ≤ k + n :=
   Nat.le_trans h (Nat.le_add_left n k)
 
-def Var := Nat deriving DecidableEq
+section cast
 
-protected def Var.toString (x : Var) : String :=
-  ⟨toString x []⟩
-where
-  toString x l :=
-    let l := Char.ofNat ('a'.toNat + x % 26) :: l
-    match h : x / 26 with
-    | 0 => l
-    | q + 1 =>
-      have := h ▸ Nat.div_le_self ..
-      toString q l
+variable {α : Sort u} {β : α → Sort v} {γ : α → Sort w}
 
-instance : ToString Var := ⟨Var.toString⟩
+@[simp]
+theorem cast_cast (h : α = α') (h' : α' = α'') (x : α) : h' ▸ h ▸ x = h.trans h' ▸ x :=
+  by cases h; rfl
 
-instance : OfNat Var n := ⟨n⟩
+@[simp]
+theorem cast_cast' (h : x = x') (h' : x' = x'') (y : β x) : h' ▸ h ▸ y = h.trans h' ▸ y :=
+  by cases h; rfl
 
-def Var.ofString : String → Var
-  | ⟨l⟩ =>
-    l.foldl (λ x c => (x + 1) * 26 + (c.toNat - 'a'.toNat).min 25) 0 - 26 ^ l.length
+@[simp]
+theorem cast_inj (h : x = x') {y y' : β x} : h ▸ y = h ▸ y' ↔ y = y' :=
+  by cases h; exact ⟨id, id⟩
 
-instance : Coe String Var := ⟨Var.ofString⟩
+theorem cast_to_cast (h : x = x') (y : β x) : h ▸ y = congrArg β h ▸ y :=
+  by cases h; rfl
+
+@[simp]
+theorem cast_app (f : ∀ x, β x → γ x) {x} (y : β x) {x'} (h : x = x') : f x' (h ▸ y) = h ▸ f x y :=
+  by cases h; rfl
+
+theorem cast_swap (hx : x = x') {y : β x} {y' : β x'} (h : hx ▸ y = y') : y = hx ▸ y' :=
+  by cases hx; cases h; rfl
+
+end cast
 
 /-
 def Var.fresh : List Var → Var
@@ -63,7 +62,7 @@ namespace Term
 
 protected def toString : Term d → String
   | fvar x => x.toString ++ "'"
-  | bvar n => Var.toString (d.pred - n.1)
+  | bvar (d := .succ d) n => Var.toString (d - n.val)
   | abs e => s!"(λ{Var.toString d}.{e.toString})"
   | app e₁ e₂ => s!"({e₁.toString} {e₂.toString})"
 
@@ -85,6 +84,13 @@ theorem weaken_refl : {e : Term d} → weaken .refl e = e
   | abs _ => congrArg abs weaken_refl
   | app .. => congrArg₂ app weaken_refl weaken_refl
 
+@[simp]
+theorem weaken_weaken (hd₁ : d₁ ≤ d₂) (hd₂ : d₂ ≤ d₃) : (e : Term d₁) → weaken hd₂ (weaken hd₁ e) = weaken (Nat.le_trans hd₁ hd₂) e
+  | fvar _ => rfl
+  | bvar _ => rfl
+  | abs e => congrArg abs (weaken_weaken (Nat.succ_le_succ hd₁) (Nat.succ_le_succ hd₂) e)
+  | app e₁ e₂ => congrArg₂ app (weaken_weaken hd₁ hd₂ e₁) (weaken_weaken hd₁ hd₂ e₂)
+
 variable (x : Var) in
 def bind : Term d → Term d.succ
   | fvar y => if y = x then bvar .last else fvar y
@@ -95,7 +101,38 @@ def bind : Term d → Term d.succ
 def abs' (x : Var) (e : Term) : Term :=
   abs (e.bind x)
 
-theorem bind_bind : bind x e = bind y e' → bind x (bind z e) = bind y (bind z e') := sorry
+/-
+theorem bind_bind (h : bind x e = bind y e') (hx : x ≠ z) (hy : y ≠ z) : bind x (bind z e) = bind y (bind z e') := by
+  induction e with
+  | fvar w =>
+    cases e'
+      <;> unfold bind at h
+      <;> split at h
+      <;> (try split at h)
+      <;> simp at h
+      <;> cases h
+      <;> simp! [*]
+    split <;> simp! [*]
+  | bvar n =>
+    cases e'
+      <;> unfold bind at h
+      <;> (try split at h)
+      <;> simp at h
+    cases h
+    rfl
+  | abs e he =>
+    cases e'
+      <;> unfold bind at h
+      <;> (try split at h)
+      <;> simp at h
+    simp! [he h]
+  | app e₁ e₂ he₁ he₂ =>
+    cases e'
+      <;> unfold bind at h
+      <;> (try split at h)
+      <;> simp at h
+    simp! [he₁ h.1, he₂ h.2]
+-/
 
 variable (e' : Term) in
 def subst : Term d.succ → Term d :=
@@ -107,11 +144,15 @@ where
   | abs e => abs (subst e)
   | app e₁ e₂ => app (subst e₁) (subst e₂)
 
-theorem subst_weaken : {e : Term d} → subst e' (weaken (.step .refl) e) = e
+theorem subst_weaken (h : d ≤ d') (e : Term d) : subst e' (weaken (.step h) e) = weaken h e :=
+  match e with
   | fvar _ => rfl
-  | bvar n => by simp [weaken, subst, subst.subst, Fin.castLe, n.2]
-  | abs _ => congrArg abs subst_weaken
-  | app .. => congrArg₂ app subst_weaken subst_weaken
+  | bvar n => by
+    dsimp [weaken, Fin.castLe, subst, subst.subst]
+    have : (n : Nat) < _ := Nat.le_trans n.2 h
+    simp [this]
+  | abs e => congrArg abs (subst_weaken (Nat.succ_le_succ h) e)
+  | app e₁ e₂ => congrArg₂ app (subst_weaken h e₁) (subst_weaken h e₂)
 
 theorem subst_bind : {e : Term d} → subst (fvar x) (bind x e) = e
   | fvar _ => by
@@ -132,6 +173,13 @@ def free : Term d → Prop
   | abs e => e.free
   | app e₁ e₂ => e₁.free ∧ e₂.free
 
+theorem bind_free (h : e.free x) : bind x e = e.weaken (.step .refl) :=
+  match e with
+  | fvar _ => if_neg h
+  | bvar _ => rfl
+  | abs _ => congrArg abs <| bind_free h
+  | app .. => congrArg₂ app (bind_free h.1) (bind_free h.2)
+
 theorem bind_subst (h : e.free x) : bind x (subst (fvar x) e) = e :=
   match e with
   | fvar _ => if_neg h
@@ -141,9 +189,15 @@ theorem bind_subst (h : e.free x) : bind x (subst (fvar x) e) = e :=
     . rfl
     next h =>
       simp [weaken, bind]
-      exact Nat.pred_le_pred n.2 |> Nat.eq_or_lt_of_le |>.resolve_right h |>.symm |> Fin.eq_of_val_eq
+      exact Nat.pred_le_pred n.2 |> Nat.eq_or_lt_of_le |>.resolve_right h |>.symm
   | abs _ => congrArg abs (bind_subst h)
   | app .. => congrArg₂ app (bind_subst h.1) (bind_subst h.2)
+
+theorem free_weaken (hd : d ≤ d') : (e : Term d) → e.free x ↔ (e.weaken hd).free x
+  | fvar _ => ⟨id, id⟩
+  | bvar _ => ⟨id, id⟩
+  | abs e => free_weaken (Nat.succ_le_succ hd) e
+  | app e₁ e₂ => ⟨λ h => ⟨free_weaken hd e₁ |>.mp h.1, free_weaken hd e₂ |>.mp h.2⟩, λ h => ⟨free_weaken hd e₁ |>.mpr h.1, free_weaken hd e₂ |>.mpr h.2⟩⟩
 
 theorem free_bind : (e : Term d) → e.free x → (e.bind y).free x
   | fvar _, h => by
@@ -155,11 +209,56 @@ theorem free_bind : (e : Term d) → e.free x → (e.bind y).free x
   | abs e, h => free_bind e h
   | app e₁ e₂, h => ⟨free_bind e₁ h.1, free_bind e₂ h.2⟩
 
+theorem free_bind' : (e : Term d) → (e.bind x).free x
+  | fvar _ => by
+    unfold bind
+    split
+    . trivial
+    . assumption
+  | bvar _ => .intro
+  | abs e => free_bind' e
+  | app e₁ e₂ => ⟨free_bind' e₁, free_bind' e₂⟩
+
+theorem of_free_bind (e : Term d) (h : (e.bind y).free x) : e.free x ∨ y = x :=
+  match e with
+  | fvar z => by
+    unfold bind at h
+    split at h
+    next h' =>
+      cases h'
+      exact Classical.em _ |>.symm
+    . exact .inl h
+  | bvar n => .inl h
+  | abs e => of_free_bind e h
+  | app e₁ e₂ =>
+    match of_free_bind e₁ h.1 with
+    | .inr h₁ => .inr h₁
+    | .inl h₁ =>
+      match of_free_bind e₂ h.2 with
+      | .inr h₂ => .inr h₂
+      | .inl h₂ => .inl ⟨h₁, h₂⟩
+
+variable {e' : Term} (h' : free x e') in
+theorem free_subst : (e : Term (.succ d)) → e.free x → (e'.subst e).free x
+  | fvar _, h => h
+  | bvar _, h => by
+    unfold subst subst.subst
+    split
+    . assumption
+    . exact free_weaken d.zero_le e' |>.mp h'
+  | abs e, h => free_subst e h
+  | app e₁ e₂, h => ⟨free_subst e₁ h.1, free_subst e₂ h.2⟩
+
 def fresh : Term d → Var
   | fvar x => x.succ
   | bvar _ => .zero
   | abs e => e.fresh
   | app e₁ e₂ => e₁.fresh.max e₂.fresh
+
+def fresh' (es : Fin k → Term d) : Var :=
+  match k with
+  | 0 => .zero
+  | _ + 1 => es .zero |>.fresh.max <| fresh' (es ·.succ')
 
 variable (x : Var) in
 theorem free_fresh (h : e.fresh.le x) : free x e :=
@@ -168,6 +267,15 @@ theorem free_fresh (h : e.fresh.le x) : free x e :=
   | bvar n => trivial
   | abs e => free_fresh (e := e) h
   | app e₁ e₂ => ⟨free_fresh <| Nat.le_trans (Nat.le_max_left ..) h, free_fresh <| Nat.le_trans (Nat.le_max_right ..) h⟩
+
+variable (x : Var) in
+theorem free_fresh' {es : Fin k → Term d} (h : fresh' es |>.le x) i : free x (es i) := by
+  induction k with
+  | zero => exact nomatch i
+  | succ k ih =>
+    cases i using Fin.cases with
+    | zero => exact free_fresh x <| Nat.le_trans (Nat.le_max_left ..) h
+    | succ i => exact ih (Nat.le_trans (Nat.le_max_right ..) h) i
 
 @[simp]
 theorem sizeOf_subst_fvar x : (e : Term d.succ) → sizeOf (subst (fvar x) e : Term d) < sizeOf e
@@ -179,6 +287,188 @@ theorem sizeOf_subst_fvar x : (e : Term d.succ) → sizeOf (subst (fvar x) e : T
     . apply Nat.le_add_right
   | abs e => Nat.add_lt_add .refl (sizeOf_subst_fvar ..)
   | app e₁ e₂ => Nat.add_lt_add (Nat.add_lt_add .refl (sizeOf_subst_fvar ..)) (sizeOf_subst_fvar ..)
+
+def bindAll (xs : Fin k → Var) {d} (e : Term d) : Term (d + k) :=
+  @Fin.rdfoldl k _ (λ k => Term (d + k)) (λ _ e x => bind x e) e xs
+
+def substAll (es : Fin k → Term) {d} (e : Term (d + k)) : Term d :=
+  @Fin.rdfoldr k _ (λ k => Term (d + k)) (λ _ e' => subst e') e es
+
+theorem substAll_bindAll {xs : Fin k → Var} {d} {e : Term d} : substAll (fvar <| xs ·) (bindAll xs e) = e := by
+  unfold substAll bindAll
+  induction k with
+  | zero => rfl
+  | succ _ ih => dsimp; rw [subst_bind]; exact ih
+
+theorem bindAll_eq_bind_bindAll {xs : Fin (.succ k) → Var} {e : Term d} : bindAll xs e = bind (xs .last) (bindAll (xs ·.castSucc) e) := rfl
+
+theorem bindAll_eq_bindAll_bind {xs : Fin (.succ k) → Var} {e : Term d} : bindAll xs e = (d.succ_add k ▸ bindAll (xs ·.succ') (bind (xs .zero) e) :) := by
+  rw [bindAll, ← Fin.dfoldl_eq_rdfoldl]
+  dsimp
+  rw [Fin.dfoldl_eq_rdfoldl, cast_to_cast]
+  refine Fin.rdfoldl_ext (congrArg @Term <| .symm <| d.succ_add ·) ?_ rfl _
+  intro i _ _
+  rw [← cast_to_cast]
+  rw [← @cast_to_cast Nat (Term ·.succ)]
+  exact cast_app _ _ <| d.succ_add i
+
+theorem bind_bindAll {xs : Fin k → Var} {e : Term d} : bind x (bindAll xs e) = bindAll (Fin.rcases xs x) e :=
+  by simp [bindAll]
+
+theorem bindAll_bind {xs : Fin k → Var} {e : Term d} : bindAll xs (bind x e) = Nat.succ_add .. ▸ bindAll (Fin.cases x xs) e :=
+  cast_swap _ <| .symm bindAll_eq_bindAll_bind
+
+@[simp]
+theorem bindAll_bvar {xs : Fin k → Var} {n : Fin d} : bindAll xs (bvar n) = bvar (n.castAdd k) := by
+  unfold bindAll
+  induction k with
+  | zero => rfl
+  | succ _ ih => exact congrArg _ ih
+
+@[simp]
+theorem bindAll_abs {xs : Fin k → Var} {e : Term (.succ d)} : bindAll xs (abs e) = abs (Nat.succ_add .. ▸ bindAll xs e) := by
+  unfold bindAll
+  induction k with
+  | zero => rfl
+  | succ _ ih => apply congrArg _ ih |>.trans; simp [bind]; rw [cast_to_cast, @cast_to_cast _ (Term <| .succ ·)]
+
+@[simp]
+theorem bindAll_app {xs : Fin k → Var} {e₁ e₂ : Term d} : bindAll xs (app e₁ e₂) = app (bindAll xs e₁) (bindAll xs e₂) := by
+  unfold bindAll
+  induction k with
+  | zero => rfl
+  | succ _ ih => exact congrArg _ ih
+
+@[simp]
+theorem bindAll_fvar_ne_abs {xs : Fin k → Var} {e : Term (d + k).succ} : bindAll xs (fvar x) ≠ abs e := by
+  unfold bindAll
+  induction k with
+  | zero => intro h; cases h
+  | succ _ ih =>
+    rw [Fin.rdfoldl]
+    generalize he' : Fin.rdfoldl .. = e'
+    cases e'
+      <;> (try unfold bind; split)
+      <;> intro h
+      <;> cases h
+    exact ih he'
+
+@[simp]
+theorem abs_ne_bindAll_fvar {xs : Fin k → Var} {e : Term (d + k).succ} : abs e ≠ bindAll xs (fvar x) :=
+  bindAll_fvar_ne_abs.symm
+
+@[simp]
+theorem bindAll_fvar_ne_app {xs : Fin k → Var} {e₁ e₂ : Term (d + k)} : bindAll xs (fvar x) ≠ app e₁ e₂ := by
+  unfold bindAll
+  induction k with
+  | zero => intro h; cases h
+  | succ _ ih =>
+    rw [Fin.rdfoldl]
+    generalize he' : Fin.rdfoldl .. = e'
+    cases e'
+      <;> (try unfold bind; split)
+      <;> intro h
+      <;> cases h
+    exact ih he'
+
+@[simp]
+theorem app_ne_bindAll_fvar {xs : Fin k → Var} {e₁ e₂ : Term (d + k)} : app e₁ e₂ ≠ bindAll xs (fvar x) :=
+  bindAll_fvar_ne_app.symm
+
+@[simp]
+theorem bindAll_fvar_ne_bvar_castAdd {xs : Fin k → Var} {n : Fin d} : bindAll xs (fvar x) ≠ bvar (n.castAdd k) := by
+  unfold bindAll
+  induction k generalizing d n with
+  | zero => intro h; cases h
+  | succ _ ih =>
+    rw [Fin.rdfoldl]
+    generalize he' : Fin.rdfoldl .. = e'
+    cases e'
+      <;> (try unfold bind; split)
+      <;> intro h
+      <;> (try cases h)
+      <;> simp [bind] at h
+    . cases Nat.ne_of_lt (Nat.le_trans n.2 <| d.le_add_right _) h.symm
+    . exact ih <| he'.trans <| congrArg bvar <| Fin.eq_of_val_eq h
+
+@[simp]
+theorem bvar_castAdd_ne_bindAll_fvar {xs : Fin k → Var} {n : Fin d} : bvar (n.castAdd k) ≠ bindAll xs (fvar x) :=
+  bindAll_fvar_ne_bvar_castAdd.symm
+
+theorem substAll_eq_substAll_subst {es : Fin (.succ k) → Term} {e : Term (d + k).succ} : substAll es e = substAll (es ·.castSucc) (subst (es .last) e) := rfl
+
+theorem substAll_eq_subst_substAll {es : Fin (.succ k) → Term} {e : Term (d + k).succ} : substAll es e = subst (es .zero) (substAll (es ·.succ') (d.succ_add k ▸ e)) := by
+  rw [substAll, ← Fin.dfoldr_eq_rdfoldr]
+  dsimp
+  congr
+  rw [Fin.dfoldr_eq_rdfoldr, cast_to_cast]
+  rw [substAll]
+  refine Fin.rdfoldr_ext (congrArg @Term <| .symm <| d.succ_add ·) ?_ (by simp) _
+  intro i _ _
+  rw [← @cast_to_cast Nat (Term ·.succ)]
+  rw [← cast_to_cast]
+  exact cast_app (@Term.subst _) _ <| d.succ_add i
+
+theorem substAll_subst {es : Fin k → Term} {e : Term (d + k).succ} : substAll es (subst e' e) = substAll (Fin.rcases es e') e :=
+  by simp [substAll]
+
+theorem subst_substAll {es : Fin k → Term} {e : Term (.succ d + k)} : subst e' (substAll es e) = substAll (Fin.cases e' es) (d.succ_add k ▸ e : Term (d + k).succ) := by
+  have := @substAll_eq_subst_substAll _ _ (Fin.cases e' es) (d.succ_add k ▸ e)
+  simp at this
+  exact this.symm
+
+@[simp]
+theorem substAll_fvar {es : Fin k → Term} : substAll es (fvar x : Term (d + k)) = fvar x := by
+  unfold substAll
+  induction k with
+  | zero => rfl
+  | succ _ ih => exact ih
+
+@[simp]
+theorem substAll_bvar_castAdd {es : Fin k → Term} {n : Fin d} : substAll es (bvar (n.castAdd k)) = bvar n := by
+  unfold substAll
+  induction k with
+  | zero => rfl
+  | succ _ ih =>
+    simp [subst, subst.subst, show (n : Nat) < _ from Nat.le_trans n.2 <| d.le_add_right _]
+    exact ih
+
+@[simp]
+theorem substAll_abs {es : Fin k → Term} {e : Term (d + k).succ} : substAll es (abs e) = abs (substAll es (Nat.succ_add .. ▸ e)) := by
+  unfold substAll
+  induction k with
+  | zero => rfl
+  | succ _ ih =>
+    apply ih.trans ∘ .symm
+    simp
+    congr
+    rw [cast_to_cast]
+    rw [← @cast_to_cast Nat (Term ·.succ)]
+    apply @cast_app Nat (Term ·.succ)
+
+@[simp]
+theorem substAll_app {es : Fin k → Term} {e₁ e₂ : Term (d + k)} : substAll es (app e₁ e₂) = app (substAll es e₁) (substAll es e₂) := by
+  unfold substAll
+  induction k with
+  | zero => rfl
+  | succ _ ih => exact ih
+
+theorem free_bindAll {xs : Fin k → Var} {e : Term d} (h : free x e) : free x (bindAll xs e) := by
+  induction k with
+  | zero => exact h
+  | succ _ ih =>
+    rw [bindAll_eq_bind_bindAll]
+    exact free_bind _ ih
+
+theorem free_substAll {es : Fin k → Term} {e : Term (d + k)} (h' : ∀ i, free x (es i)) (h : free x e) : free x (substAll es e) := by
+  induction k generalizing d with
+  | zero => exact h
+  | succ _ ih =>
+    rw [substAll_eq_subst_substAll]
+    apply free_subst (h' .zero)
+    apply ih (h' ·.succ')
+    simp
+    exact h
 
 section Congruence
 
@@ -204,14 +494,14 @@ inductive CongruenceClosure : Term → Term → Prop
 instance CongruenceClosure.instCongruence : Congruence (CongruenceClosure r) := ⟨@abs r, @app₁ r, @app₂ r⟩
 
 instance ReflexiveTransitiveClosure.instCongruence [Congruence r] : Congruence (ReflexiveTransitiveClosure r) where
-  abs := ReflexiveTransitiveClosure.lift (Congruence.abs ·)
-  app₁ := ReflexiveTransitiveClosure.lift (Congruence.app₁ ·)
-  app₂ := ReflexiveTransitiveClosure.lift (Congruence.app₂ ·)
+  abs := ReflexiveTransitiveClosure.map' (Congruence.abs ·)
+  app₁ := ReflexiveTransitiveClosure.map' (Congruence.app₁ ·)
+  app₂ := ReflexiveTransitiveClosure.map' (Congruence.app₂ ·)
 
 instance EquivalenceClosure.instCongruence [Congruence r] : Congruence (EquivalenceClosure r) where
-  abs := EquivalenceClosure.lift (Congruence.abs ·)
-  app₁ := EquivalenceClosure.lift (Congruence.app₁ ·)
-  app₂ := EquivalenceClosure.lift (Congruence.app₂ ·)
+  abs := EquivalenceClosure.map' (Congruence.abs ·)
+  app₁ := EquivalenceClosure.map' (Congruence.app₁ ·)
+  app₂ := EquivalenceClosure.map' (Congruence.app₂ ·)
 
 end Congruence
 
@@ -234,8 +524,8 @@ def Θ := reduce%
 #eval Θ
 
 example : Θ f ↠β f (Θ f) :=
-  .trans (.base <| .app₁ <| .base .β) <|
-  .trans (.base <| .base .β) <|
+  .trans (.base <| .app₁ <| .base .β') <|
+  .trans (.base <| .base .β') <|
   Reflexive.ofEq <|
   congrArg₂ app weaken_refl <| congrArg₂ app rfl weaken_refl
 
@@ -245,9 +535,9 @@ def Y := reduce%
 #eval Y
 
 example : Y f =β f (Y f) :=
-  .trans (.base <| .base .β) <|
-  .trans (.base <| .base .β) <|
-  flip .trans (.symm <| .base <| .app₂ <| .base .β) <|
+  .trans (.base <| .base .β') <|
+  .trans (.base <| .base .β') <|
+  flip .trans (.symm <| .base <| .app₂ <| .base .β') <|
   Reflexive.ofEq <|
   congrArg₂ app subst_weaken <| congrArg₂ app weaken_refl weaken_refl
 -/
@@ -256,7 +546,7 @@ namespace Confluence
 
 inductive BetaParallel : Term → Term → Prop
   | β : BetaParallel e₁ e₁' → BetaParallel e₂ e₂' → BetaParallel (app (abs' x e₁) e₂) (e₂'.subst (e₁'.bind x))
-  | var : BetaParallel (fvar x) (fvar x) -- TODO : change this to refl
+  | var : BetaParallel (fvar x) (fvar x)
   | abs : BetaParallel e e' → BetaParallel (abs' x e) (abs' x e')
   | app : BetaParallel e₁ e₁' → BetaParallel e₂ e₂' → BetaParallel (app e₁ e₂) (.app e₁' e₂')
 
@@ -265,57 +555,36 @@ infix:50 " ▷β* " => ReflexiveTransitiveClosure BetaParallel
 
 namespace BetaParallel
 
-theorem abs' (h : let x := fvar (e.fresh.max e'.fresh); x.subst e ▷β x.subst e') : .abs e ▷β .abs e' :=
-  abs h |> (congrArg₂ BetaParallel · · |>.mp)
-    (congrArg _ <| bind_subst <| free_fresh _ <| Nat.le_max_left ..)
-    (congrArg _ <| bind_subst <| free_fresh _ <| Nat.le_max_right ..)
+theorem abs' (hx : e.free x) (hx' : e'.free x) (h : (fvar x).subst e ▷β (fvar x).subst e') : .abs e ▷β .abs e' :=
+  bind_subst hx ▸ bind_subst hx' ▸ abs h
 
-theorem refl : ∀ {e}, e ▷β e
-  | .fvar _ => var
+theorem abs'' (h : let x := fvar (e.fresh.max e'.fresh); x.subst e ▷β x.subst e') : .abs e ▷β .abs e' :=
+  abs' (free_fresh _ <| Nat.le_max_left ..) (free_fresh _ <| Nat.le_max_right ..) h
+
+theorem refl : ∀ {e}, BetaParallel e e
+  | fvar x => var
   | .abs e =>
-    have := sizeOf_subst_fvar (e.fresh.max e.fresh) e
-    have := Nat.le_trans this <| Nat.le_add_left _ 1
-    abs' refl
-  | .app _ _ => app refl refl
-termination_by _ e => e
+    have := Nat.le_trans (sizeOf_subst_fvar (e.fresh.max e.fresh) e) <| Nat.le_add_left _ 1
+    abs'' refl
+  | .app .. => app refl refl
 
-theorem red : e →β e' → e ▷β e'
+theorem ofBetaReduction : e →β e' → e ▷β e'
   | .base .β => β refl refl
-  | .abs h => abs (red h)
-  | .app₁ h => app (red h) refl
-  | .app₂ h => app refl (red h)
+  | .abs h => abs (ofBetaReduction h)
+  | .app₁ h => app (ofBetaReduction h) refl
+  | .app₂ h => app refl (ofBetaReduction h)
 
-theorem red_t : e ▷β e' → e ↠β e'
-  | β h₁ h₂ => .trans (.trans (Congruence.app₁ <| Congruence.abs <| red_t h₁) (Congruence.app₂ <| red_t h₂)) (.base <| .base .β)
+theorem toBetaReduction : e ▷β e' → e ↠β e'
+  | β h₁ h₂ => .trans (.trans (Congruence.app₁ <| Congruence.abs <| toBetaReduction h₁) (Congruence.app₂ <| toBetaReduction h₂)) (.base <| .base .β)
   | var => .refl
-  | abs h => Congruence.abs <| red_t h
-  | app h₁ h₂ => .trans (Congruence.app₁ <| red_t h₁) (Congruence.app₂ <| red_t h₂)
+  | abs h => Congruence.abs <| toBetaReduction h
+  | app h₁ h₂ => .trans (Congruence.app₁ <| toBetaReduction h₁) (Congruence.app₂ <| toBetaReduction h₂)
 
-theorem clos₁ : e ↠β e' → e ▷β* e' :=
-  .lift (r := CongruenceClosure _) red
+theorem multiOfBetaReduction : e ↠β e' → e ▷β* e' :=
+  .map' (r := CongruenceClosure _) ofBetaReduction
 
-theorem clos₂ (h : e ▷β* e') : e ↠β e' :=
-  h.rec red_t .refl λ _ _ => .trans
-
-/-
-theorem lift {M M' : Term f} {b : Fin2 f.succ} : M ▷β M' → M.lift' b.toNat ▷β M'.lift' b.toNat
-  | β h₁ h₂ => Term.lift'_subst _ _ b ▸ .β (Fin2.toNat_castSucc ▸ lift h₁) (lift h₂)
-  | var => var
-  | abs h => abs (Fin2.toNat_castSucc ▸ lift h)
-  | app h₁ h₂ => app (lift h₁) (lift h₂)
-
-theorem subst {M M' : Term (.succ f)} {N N' : Term f} (hN : N ▷β N') : M ▷β M' → ∀ {b}, M.subst' b N ▷β M'.subst' b N'
-  | β _ _, .zero => (sorry : .app (.abs (.subst' _ .zero N.lift)) (.subst' _ .zero N) ▷β .subst' (.subst _ _) .zero N')
-  | β _ _, .succ b => (sorry : .app (.abs (.subst' _ b.castSucc.succ N.lift)) (.subst' _ b.succ N) ▷β .subst' (.subst _ _) b.succ N')
-    | @var _ n, b => by
-    simp [Term.subst'.impl, Term.impl.subst']
-    cases Term.substVar b n <;> simp
-    case zero => exact hN
-    case succ => exact var
-  | abs h, .zero => abs (subst (by have := @lift _ _ _ (@Fin2.last f) hN; simp at this; exact this : N.lift' f ▷β N'.lift' f) h)
-  | abs h, .succ b => abs (subst (by have := @lift _ _ _ (@Fin2.last f) hN; simp at this; exact this : N.lift ▷β N'.lift) h)
-  | app h₁ h₂, _ => app (subst hN h₁) (subst hN h₂)
--/
+theorem multiToBetaReduction : e ▷β* e' → e ↠β e' :=
+  .map (r := BetaParallel) toBetaReduction
 
 end BetaParallel
 
@@ -325,16 +594,468 @@ inductive MaxBeta : Term → Term → Prop
   | abs : MaxBeta e e' → MaxBeta (abs' x e) (abs' x e')
   | app : (∀ e₁', e₁ ≠ abs e₁') → MaxBeta e₁ e₁' → MaxBeta e₂ e₂' → MaxBeta (app e₁ e₂) (.app e₁' e₂')
 
-theorem MaxBeta.deterministic : ∀ e, MaxBeta e e₁ → MaxBeta e e₂ → e₁ = e₂
-  | .fvar _, .var, .var => rfl
-  | .abs e, h, h' => by
-    generalize he' : e = e' at h'
-    cases h with | abs h =>
-    cases h' with | abs h' =>
-    apply congrArg Term.abs
+/-
+@[simp]
+theorem cast_cast {α : Sort u} {β : α → Sort v} {x₁ x₂ x₃ : α} (h₁ : x₁ = x₂) (h₂ : x₂ = x₃) (y : β x₁) : h₂ ▸ h₁ ▸ y = h₁.trans h₂ ▸ y := by
+  subst_eqs
+  rfl
+
+theorem cast_cast' {α : Sort u} {α' : Sort v} {β : α → Sort w} {β' : α' → Sort w} {x₁ x₂ : α} {x₂' x₃' : α'} (h₁ : x₁ = x₂) (h : β x₂ = β' x₂') (h₂ : x₂' = x₃') (y : β x₁) : h₂ ▸ h ▸ h₁ ▸ y = (congrArg β h₁ |>.trans h |>.trans (congrArg β' h₂)) ▸ y := by
+  subst_eqs
+  rfl
+-/
+
+theorem _root_.Term.bindAll_weaken_eq {l l' : Fin k → Var} {e e' : Term d} (h : e.bindAll l = e'.bindAll l') (hd : d ≤ d') : bindAll l (weaken hd e) = bindAll l' (weaken hd e') := by
+  induction e generalizing d'
+    <;> cases e'
+    <;> simp at h
+    <;> (try cases h)
+    <;> simp! [*]
+  case fvar =>
+    clear d hd
+    rename_i d x y
+    induction k generalizing d d' with
+    | zero => cases h; rfl
+    | succ k ih =>
+      simp [bindAll_eq_bindAll_bind, bind] at h ⊢
+      split
+        <;> split
+        <;> simp [*] at h
+      . simp
+      . exact ih h
+  case abs ih _ => exact ih h _
+  case app ih₁ ih₂ _ _ h₁ h₂ => exact ⟨ih₁ h₁ _, ih₂ h₂ _⟩
+
+theorem _root_.Term.bindAll_eq_of_weaken {l l' : Fin k → Var} {e e' : Term d} (hd : d ≤ d') (h : bindAll l (weaken hd e) = bindAll l' (weaken hd e')) : bindAll l e = bindAll l' e' := by
+  induction e generalizing d'
+    <;> cases e'
+    <;> simp! at h
+    <;> (try cases h)
+    <;> simp [*]
+  case fvar.bvar n => cases bindAll_fvar_ne_bvar_castAdd (n := n.castLe hd) h
+  case bvar.fvar n _ => cases bvar_castAdd_ne_bindAll_fvar (n := n.castLe hd) h
+  case fvar =>
+    clear d hd
+    rename_i d x y
+    induction k generalizing d d' with
+    | zero => cases h; rfl
+    | succ k ih =>
+      simp [bindAll_eq_bindAll_bind, bind] at h ⊢
+      split
+        <;> split
+        <;> simp [*] at h
+      . simp
+      . exact ih h
+  case abs ih _ => exact ih _ h
+  case app ih₁ ih₂ _ _ h₁ h₂ => exact ⟨ih₁ _ h₁, ih₂ _ h₂⟩
+
+theorem _root_.Term.bindAll_subst_bind (l l' : Fin k → Var) {e₁ e₁' : Term d} {e₂ e₂' : Term} {x y : Var} (h₁ : bindAll l (e₁.bind x) = bindAll l' (e₁'.bind y)) (h₂ : bindAll l e₂ = bindAll l' e₂') : bindAll l (e₂.subst (e₁.bind x)) = bindAll l' (e₂'.subst (e₁'.bind y)) := by
+  induction e₁ with
+  | fvar z =>
+    cases e₁' with
+    | fvar w =>
+      dsimp [bind] at h₁ ⊢
+      split
+        <;> split
+        <;> rename_i heq₁ heq₂
+        <;> simp [heq₁, heq₂] at h₁
+        <;> simp [subst, subst.subst, Fin.last]
+      . exact bindAll_weaken_eq h₂ (Nat.zero_le _)
+      . exact bindAll_eq_of_weaken (Nat.le_succ _) h₁
+    | bvar n =>
+      simp! at h₁
+      split at h₁
+      . simp [Fin.castLe, Fin.last, Nat.ne_of_lt n.2 |>.symm] at h₁
+      . cases bindAll_fvar_ne_bvar_castAdd (n := n.castSucc) h₁
+    | abs => simp! at h₁; split at h₁ <;> simp at h₁
+    | app => simp! at h₁; split at h₁ <;> simp at h₁
+  | bvar n =>
+    cases e₁' with
+    | fvar x =>
+      simp! at h₁
+      split at h₁
+      . simp [Fin.castLe, Fin.last, Nat.ne_of_lt n.2] at h₁
+      . cases bindAll_fvar_ne_bvar_castAdd (n := n.castSucc) h₁.symm
+    | bvar n' =>
+      simp! at h₁
+      dsimp [Fin.castLe] at h₁
+      cases Fin.eq_of_val_eq h₁
+      simp [subst, subst.subst, Fin.castSucc, n.2]
+    | abs => simp! at h₁
+    | app => simp! at h₁
+  | abs _ h =>
+    cases e₁' with
+    | fvar => simp! at h₁; split at h₁; simp at h₁; have := h₁.symm; simp at this
+    | bvar => simp! at h₁
+    | abs => simp [bind, subst, subst.subst] at h₁ ⊢; exact h h₁
+    | app => simp! at h₁
+  | app _ _ h h' =>
+    cases e₁' with
+    | fvar => simp! at h₁; split at h₁; simp at h₁; have := h₁.symm; simp at this
+    | bvar => simp! at h₁
+    | abs => simp! at h₁
+    | app => simp [bind, subst, subst.subst] at h₁ ⊢; exact ⟨h h₁.1, h' h₁.2⟩
+
+theorem free_beta (h : e.free x) (h' : e →β e') : e'.free x := by
+  induction h' with
+  | base h' =>
+    cases h'
+    exact free_subst h.2 _ h.1
+  | abs h' ih =>
+    cases of_free_bind _ h with
+    | inl h' => exact free_bind _ <| ih h'
+    | inr h' => cases h'; exact free_bind' _
+  | app₁ _ ih => exact ⟨ih h.1, h.2⟩
+  | app₂ _ ih => exact ⟨h.1, ih h.2⟩
+
+theorem subst_bind_weaken (hd : d ≤ d') : subst e' (bind x (weaken hd e)) = weaken hd (subst e' (bind x e)) := by
+  induction e generalizing d' with
+  | fvar =>
+    dsimp [weaken, bind]
+    split
+    . simp [subst, subst.subst]
+    . rfl
+  | bvar n =>
+    dsimp [bind, subst, subst.subst]
+    simp [n.2, show n < d' from Nat.le_trans n.2 hd]
+    rfl
+  | abs _ ih => exact congrArg abs <| ih <| Nat.succ_le_succ hd
+  | app _ _ ih₁ ih₂ => exact congrArg₂ app (ih₁ hd) (ih₂ hd)
+
+theorem subst_bind_subst_bind (h : free x e₂) (hx : x ≠ y) : subst e₂ (bind y (subst e₁ (bind x e))) = subst (subst e₂ (bind y e₁)) (bind x (subst e₂ (bind y e))) := by
+  induction e with
+  | fvar =>
+    dsimp [bind]
+    split
+    . subst_eqs
+      simp [hx, bind, subst, subst.subst]
+      apply subst_bind_weaken
+    . dsimp [bind]
+      split
+      . simp [subst, subst.subst]
+        rw [bind_free <| free_weaken _ e₂ |>.mp h]
+        simp
+        rw [← subst]
+        rw [subst_weaken]
+      . simp [*, bind, subst, subst.subst]
+  | bvar n => simp [bind, subst, subst.subst, n.2]
+  | abs _ ih => exact congrArg abs ih
+  | app _ _ ih₁ ih₂ => exact congrArg₂ app ih₁ ih₂
+
+theorem subst_bind_subst_bind' : subst e₂ (bind x (subst e₁ (bind x e))) = subst (subst e₂ (bind x e₁)) (bind x e) := by
+  induction e with
+  | fvar =>
+    dsimp [bind]
+    split
+    . simp [subst, subst.subst]
+      apply subst_bind_weaken
+    . simp [subst, subst.subst, bind, *]
+  | bvar n => simp [bind, subst, subst.subst, n.2]
+  | abs _ ih => exact congrArg abs ih
+  | app _ _ ih₁ ih₂ => exact congrArg₂ app ih₁ ih₂
+
+theorem subst_bind_bind (h : x ≠ y) (h' : free x e') : subst e' (bind y (bind x e)) = bind x (subst e' (bind y e)) := by
+  induction e with
+  | fvar =>
+    dsimp!
+    split
+    . subst_eqs
+      simp [h, bind, subst, subst.subst]
+    . split
+      . simp [bind, *, subst, subst.subst]
+        rw [bind_free <| free_weaken (Nat.zero_le _) _ |>.mp h']
+        simp
+      . simp [bind, *]
+        rfl
+  | bvar n => simp [bind, subst, subst.subst, n.2, Nat.lt.step n.2]
+  | abs _ ih => exact congrArg abs ih
+  | app _ _ ih₁ ih₂ => exact congrArg₂ app ih₁ ih₂
+
+example (h : e →β e') : subst e'' (bind x e) →β subst e'' (bind x e') := by
+  induction h with
+  | @base e e' h =>
+    rename_i A B; clear A B
+    cases h with | @β y e₁ e₂ =>
+    refine .base ?_
+    dsimp [abs', bind, subst, subst.subst]
+    by_cases y = x
+    next h =>
+      cases h
+      rw [bind_free (free_bind' e₁)]
+      rw [← subst, ← subst, ← subst]
+      rw [subst_weaken .refl, weaken_refl]
+      rw [subst_bind_subst_bind']
+      exact .β
+    next h =>
+      rw [← subst, ← subst, ← subst]
+      let z : Var := e₁.fresh.max e''.fresh |>.max x.succ
+      have he₁ : free z e₁ := free_fresh z <| Nat.le_trans (Nat.le_max_left ..) <| Nat.le_max_left ..
+      have he'' : free z e'' := free_fresh z <| Nat.le_trans (Nat.le_max_right ..) <| Nat.le_max_left ..
+      have hx : z ≠ x := Ne.symm <| Nat.ne_of_lt <| Nat.le_max_right ..
+      rw [← @bind_subst z _ (bind y e₁) (free_bind _ he₁)]
+      rw [subst_bind_bind hx he'']
+      conv => rhs; rw [subst_bind_subst_bind he'' hx]
+      exact .β
+  | @abs y e e' h ih =>
+    dsimp [abs', bind, subst, subst.subst]
+    rw [← subst]
+    let z : Var := e.fresh.max e''.fresh |>.max x.succ
+    have he : free z e := free_fresh z <| Nat.le_trans (Nat.le_max_left ..) <| Nat.le_max_left ..
+    have he'' : free z e'' := free_fresh z <| Nat.le_trans (Nat.le_max_right ..) <| Nat.le_max_left ..
+    have hx : z ≠ x := Ne.symm <| Nat.ne_of_lt <| Nat.le_max_right ..
+    rw [← @bind_subst z _ (bind y e) (free_bind _ he)]
+    rw [← @bind_subst z _ (bind y e') (free_bind _ <| free_beta he h)]
+    rw [subst_bind_bind hx he'']
+    rw [subst_bind_bind hx he'']
+    refine .abs ?_
     sorry
-  | .app e₁ e₂, .app _ h₁ h₂, .app _ h₁' h₂' => by cases deterministic e₁ h₁ h₁'; cases deterministic e₂ h₂ h₂'; rfl
-  | .app (.abs' x e₁) e₂, .β h₁ h₂, .β h₁' h₂' => by cases deterministic e₁ h₁ h₁'; cases deterministic e₂ h₂ h₂'; rfl
+  | app₁ _ ih => exact .app₁ ih
+  | app₂ _ ih => exact .app₂ ih
+
+theorem substAll_bindAll_weaken {xs : Fin k → Var} (hd : d ≤ d') : substAll es (bindAll xs (weaken hd e)) = weaken hd (substAll es (bindAll xs e)) := by
+  induction e generalizing d' with
+  | fvar =>
+    dsimp [weaken]
+    induction k generalizing d' with
+    | zero => rfl
+    | succ k ih =>
+      simp [bindAll_eq_bindAll_bind, substAll_eq_subst_substAll, bind]
+      split
+      . simp [subst, subst.subst]
+      . rw [ih hd.step]
+        rw [subst_weaken hd]
+        congr
+        conv => rhs; rw [ih (.step .refl)]
+        rw [subst_weaken .refl]
+        rw [weaken_refl]
+  | bvar n =>
+    simp!
+    exact substAll_bvar_castAdd (n := n.castLe hd)
+  | abs _ ih => simp!; exact ih <| Nat.succ_le_succ hd
+  | app _ _ ih₁ ih₂ => simp!; exact ⟨ih₁ hd, ih₂ hd⟩
+
+/-
+theorem substAll_bindAll_bind {e : Term d} (hi : ∀ i, (es i).free x) : ((e.bind x).bindAll xs).substAll es = ((e.bindAll xs).substAll es).bind x := by
+  induction e with
+  | fvar _ =>
+    dsimp!
+    split
+    . simp; sorry
+    . apply Eq.symm
+      apply Eq.trans
+      . apply bind_free
+        apply free_substAll hi
+        apply free_bindAll
+        assumption
+      . sorry
+  | bvar _ => simp!; sorry
+  | abs _ ih => simp!; exact ih
+  | app _ _ ih₁ ih₂ => simp!; exact ⟨ih₁, ih₂⟩
+-/
+
+example {xs : Fin k → Var} (h : e →β e') : (e.bindAll xs).substAll es →β (e'.bindAll xs).substAll es := by
+  induction h generalizing k with
+  | @base e e' h =>
+    refine .base ?_
+    rename_i A B; clear A B
+    cases h with | @β x e₁ e₂ =>
+    simp [abs']
+    induction k generalizing x e₁ e₂ with
+    | zero => exact .β
+    | succ k ih =>
+      simp [bindAll_eq_bindAll_bind, substAll_eq_subst_substAll]
+      by_cases xs .zero = x
+      next h =>
+        cases h
+        rw [bind_free <| free_bind' e₁]
+        rw [substAll_bindAll_weaken]
+        rw [subst_weaken .refl]
+        rw [weaken_refl]
+        specialize @ih (es ·.succ') (xs ·.succ') (xs .zero) e₁
+        sorry
+      next h =>
+        sorry
+    /-
+    have := @BetaReduction.β x (e₁.bindAll xs |>.substAll es) (e₂.bindAll xs |>.substAll es)
+    dsimp [abs'] at this
+    rw [substAll_bindAll_bind]
+    sorry
+    sorry
+    -/
+  | @abs x e e' h ih =>
+    simp [abs']
+    let y := fresh' (Fin.cases e es)
+    refine Congruence.abs' (x := y) (free_substAll (free_fresh' y <| Nat.le_max_right ..) <| free_bindAll <| free_bind e <| free_fresh' y .refl .zero) (free_substAll (free_fresh' y <| Nat.le_max_right ..) <| free_bindAll <| free_bind e' <| free_beta (free_fresh' y .refl .zero) h) ?_
+    simp [bindAll_bind, subst_substAll]
+    sorry
+  | app₁ _ ih => simp; exact .app₁ ih
+  | app₂ _ ih => simp; exact .app₂ ih
+
+theorem BetaParallel.ofAbs' (h : .abs e ▷β .abs e') : ∃ x, (fvar x).subst e ▷β (fvar x).subst e' := by
+  generalize h₁ : Term.abs e = e₁ at h
+  generalize h₂ : Term.abs e' = e₂ at h
+  cases h with
+  | β => cases h₁
+  | var => cases h₁
+  | app => cases h₁
+  | @abs _ _ x =>
+  cases h₁
+  cases h₂
+  apply Exists.intro x
+  rw [subst_bind]
+  rw [subst_bind]
+  assumption
+
+theorem BetaParallel.indep {xs : Fin k → Var} {l l' : Fin k → Term} (hl : ∀ i, l i ▷β l' i) (h : (e.bindAll xs).substAll l ▷β (e'.bindAll xs).substAll l') : e ▷β e' := by
+  match e with
+  | fvar x =>
+    simp only [bindAll_eq_bindAll'] at h
+    induction k with
+    | zero => exact h
+    | succ k ih =>
+      dsimp! at h
+      specialize @ih (xs ·.castSucc) (l ·.castSucc) (l' ·.castSucc) (hl ·.castSucc)
+      sorry
+  | .abs e =>
+    sorry
+  | .app e₁ e₂ =>
+    sorry
+
+theorem BetaParallel.ofAbs (h : .abs' x e ▷β .abs' x e') : e ▷β e' := by
+  have := ofAbs' h
+  clear h
+  rename _ => h
+  cases h with | _ x' h =>
+  exact indep (k := 1) (xs := λ _ => x) (λ _ => var) h
+
+theorem BetaParallel.subst₁ {es es' : Fin k → Term} (he : ∀ i, es i ▷β es' i) (h : e ▷β e') : (e.bindAll xs).substAll es ▷β (e'.bindAll xs).substAll es' := by
+  rw [bindAll_eq_bindAll']
+  induction k with
+  | zero => exact h
+  | succ k ih =>
+    dsimp!
+    sorry
+
+theorem BetaParallel.subst (h₁ : e₁ ▷β e₁') (h₂ : e₂ ▷β e₂') : e₂.subst (e₁.bind x) ▷β e₂'.subst (e₁'.bind x) := by
+  dsimp!
+  sorry
+
+theorem MaxBeta.indep {l l' : Fin k → Var} (h : e₁.bindAll l = e₂.bindAll l') (h₁ : MaxBeta e₁ e₁') (h₂ : MaxBeta e₂ e₂') : e₁'.bindAll l = e₂'.bindAll l' :=
+  match e₁ with
+  | fvar x =>
+    match e₂ with
+    | fvar y =>
+      match h₁, h₂ with
+      | .var, .var => h
+    | .abs _ => by simp at h
+    | .app .. => by simp at h
+  | .abs e₁ =>
+    match e₂ with
+    | fvar x => have := h.symm; by simp at this
+    | .abs e₂ =>
+      match ph₁ : h₁, h₂ with
+      | @abs ne₁ e₁' x h₁, @abs e₂ e₂' y h₂ => by
+        simp [abs']
+        simp [bindAll_bind] at h ⊢
+        have : sizeOf ne₁ < 1 + sizeOf e₁ := by
+          rename e₁ = _ => pe₁
+          rw [pe₁]
+          clear k l l' h₁ e₂ e₂' y h₂ pe₁ ph₁ h
+          rename_i A B C D
+          clear A B C e₂' e₁ h₁ e₂ h₂ e₁' D
+          generalize Nat.zero = d at ne₁
+          induction ne₁ with
+          | fvar => dsimp!; split <;> decreasing_tactic
+          | bvar =>
+            dsimp!
+            dsimp [Fin.castSucc, sizeOf, Fin._sizeOf_1]
+            decreasing_tactic
+          | abs _ he =>
+            dsimp!
+            apply Nat.lt_trans
+            apply Nat.add_lt_add_left he
+            decreasing_tactic
+          | app _ _ he₁ he₂ =>
+            dsimp!
+            apply Nat.le_trans
+            apply Nat.add_le_add_left he₂
+            apply Nat.le_trans
+            rw [Nat.add_assoc]
+            apply Nat.add_le_add_left
+            apply Nat.add_le_add_right
+            rw [Nat.succ_add] at he₁
+            exact Nat.le_of_succ_le_succ he₁
+            decreasing_tactic
+        exact indep (e₁ := ne₁) h h₁ h₂
+    | .app .. => by simp at h
+  | .app e₁ e₁' =>
+    match e₂ with
+    | fvar x => have := h.symm; by simp at this
+    | .abs _ => by simp at h
+    | .app e₂ e₂' =>
+      match ph₁ : h₁ with
+      | @β A E₁ _ E₂ x ha hb =>
+        match h₂ with
+        | @β B E₁' _ E₂' y hc hd => by
+          simp [abs', bindAll_bind] at h
+          apply bindAll_subst_bind l l'
+          . have : sizeOf A < 1 + sizeOf e₁ + sizeOf e₁' := by
+              rename e₁ = _ => pe₁
+              rw [pe₁]
+              apply Nat.lt_add_right
+              clear k l l' e₁ e₁' h₁ e₂ e₂' h₂ ha hb pe₁ ph₁ B E₁' E₂' y hc hd h
+              rename_i A
+              clear e₁ e₁' e₂ e₂' E₁ E₂ A
+              dsimp [abs']
+              suffices ∀ d (A : Term d), sizeOf A < 1 + (1 + sizeOf (bind x A)) from this _ A
+              clear A
+              intro d A
+              induction A with
+              | fvar =>
+                dsimp!
+                split <;> decreasing_tactic
+              | bvar =>
+                dsimp!
+                dsimp [Fin.castSucc, sizeOf, Fin._sizeOf_1]
+                decreasing_tactic
+              | abs _ he =>
+                dsimp!
+                apply Nat.lt_trans
+                apply Nat.add_lt_add_left he
+                decreasing_tactic
+              | app _ _ he₁ he₂ =>
+                dsimp!
+                apply Nat.le_trans
+                apply Nat.add_le_add_left he₂
+                apply Nat.le_trans
+                rw [Nat.add_assoc]
+                apply Nat.add_le_add_left
+                apply Nat.add_le_add_right
+                rw [Nat.succ_add] at he₁
+                exact Nat.le_of_succ_le_succ he₁
+                decreasing_tactic
+            have := indep (e₁ := A) h.1 ha hc
+            simp! at this
+            exact this
+          . exact indep (e₁ := e₁') h.2 hb hd
+        | app happ .. =>
+          match e₂ with
+          | fvar _ => by simp [abs'] at h
+          | .abs _ => by cases happ _ rfl
+          | .app .. => by simp [abs'] at h
+      | app happ ha hb =>
+        match h₂ with
+        | β .. =>
+          match e₁ with
+          | fvar _ => by simp [abs'] at h
+          | .abs _ => by cases happ _ rfl
+          | .app .. => by simp [abs'] at h
+        | app _ hc hd => by
+          simp at h ⊢
+          exact ⟨indep h.1 ha hc, indep h.2 hb hd⟩
+
+theorem MaxBeta.deterministic : MaxBeta e e₁ → MaxBeta e e₂ → e₁ = e₂ :=
+  indep (l := Fin.elim) (l' := Fin.elim) rfl
 
 def maxBeta : Term → Term
   | .fvar x => .fvar x
@@ -371,103 +1092,43 @@ theorem MaxBeta_maxBeta : ∀ e, MaxBeta e (maxBeta e)
     simp [maxBeta]
     exact .app (λ _ h => nomatch h) (MaxBeta_maxBeta _) (MaxBeta_maxBeta e₂)
 
-theorem maxBeta_subst : (e : Term 1) → e.free x → e.free y → (maxBeta ((fvar x).subst e)).bind x = (maxBeta ((fvar y).subst e)).bind y
-  | .fvar z, hx, hy => by unfold free at hx hy; simp [bind, hx, hy]
-  | .bvar .zero, hx, hy => by simp [bind]
-  | .abs e, hx, hy => by
-    unfold free at hx hy
-    simp [subst, subst.subst, fresh, maxBeta, Term.abs', bind]
-    have := maxBeta_subst (x := ((fvar x).subst e).fresh) ((fvar x).subst e) (free_fresh _ .refl) (free_fresh (fresh (subst (fvar y) e)) sorry)
-    simp [subst] at this
-    rw [this]
-    sorry
-  | .app (.abs e₁) e₂, hx, hy => sorry
-  | .app e₁ e₂, hx, hy => sorry
+theorem maxBeta_abs' : maxBeta (abs' x e) = .abs' x (maxBeta e) := by
+  have he₁ := MaxBeta_maxBeta (abs' x e)
+  generalize maxBeta _ = e₁ at he₁
+  have he₂ := MaxBeta_maxBeta e
+  generalize maxBeta e = e₂ at he₂
+  exact MaxBeta.deterministic he₁ <| MaxBeta.abs he₂
 
-/-
-theorem maxBeta_free : ∀ e : Term, (e.bind x).free y → (maxBeta ((fvar y).subst (e.bind x))).bind y = (maxBeta e).bind x
-  | .fvar x, h => by
-    dsimp [bind]
-    split
-    . simp [bind]
-    next h' =>
-      simp [bind, free, h'] at h
-      simp [bind, h]
-  | .abs e, h => by
-    --have := maxBeta_free (x := sorry) ((fvar sorry).subst e) sorry
-    simp [bind, fresh, subst, maxBeta]
-    sorry
-  | .app (.abs e₁) e₂, h => by
-    sorry
-  | .app e₁ e₂, h => sorry
-
-theorem maxBeta_abs' : ∀ e, maxBeta (Term.abs' x e) = .abs' x (maxBeta e) := by
-  intro e
-  simp [Term.abs', maxBeta]
-  apply maxBeta_free e <| free_fresh _ .refl
-/-
-  | .fvar x => by
-    simp [Term.abs', maxBeta, bind]
-    split
-    . simp [bind]
-    . simp [bind, fresh]
-  | .abs e => by
-    simp [Term.abs', maxBeta, bind, subst, fresh, weaken]
-    have := maxBeta_abs' (x := x) ((fvar e.fresh).subst e)
-    simp [Term.abs', maxBeta, bind, subst, fresh, weaken] at this
-    sorry
-  | .app (.abs e₁) e₂ => by
-    simp [Term.abs', maxBeta]
-    sorry
-  | .app e₁ e₂ => sorry
-  -/
-  -/
-
-theorem maxBeta.max : M ▷β M' → M' ▷β maxBeta M
-  | .β h₁ h₂ => sorry -- .subst (max h₂) (max h₁)
-  | .var => .var
-  | .abs (x := x) h => /-show _ ▷β maxBeta (Term.abs _) from by
-    unfold maxBeta
-    dsimp
-    apply Eq.mp (congrArg ..) <| BetaParallel.abs (x := x) (max h)
-    apply congrArg Term.abs
-    sorry-/
-    sorry
-  | .app h₁ h₂ =>
+theorem maxBeta.max (h : M ▷β M') : M' ▷β maxBeta M := by
+  induction h with
+  | β _ _ ih₁ ih₂ =>
+    rename_i e₁ e₁' e₂ e₂' x h₁ h₂
+    have her := MaxBeta_maxBeta (app (abs' x e₁) e₂)
+    generalize maxBeta _ = er at her
+    have : MaxBeta ((app (abs' x e₁) e₂)) (subst (maxBeta e₂) (bind x (maxBeta e₁))) := .β (MaxBeta_maxBeta _) (MaxBeta_maxBeta _)
+    cases her.deterministic this
+    exact .subst ih₁ ih₂
+  | var => exact .var
+  | abs h ih => rw [maxBeta_abs']; exact .abs ih
+  | app h₁ _ ih₁ ih₂ =>
     match h₁ with
-    | .β h₁ h₁' => .app (max (.β h₁ h₁')) (max h₂)
-    | .var => .app (max .var) (max h₂)
-    | .app h₁ h₁' => .app (max (.app h₁ h₁')) (max h₂)
-    | .abs h₁ => .β (max h₁) (max h₂)
+    | .abs h₁ =>
+      rename_i A B e₂ e₂' E h₁ e₁ e₁' x
+      clear M M' A B E
+      rw [maxBeta_abs'] at ih₁
+      have her := MaxBeta_maxBeta (app (abs' x e₁) e₂)
+      generalize maxBeta _ = er at her
+      have : MaxBeta ((app (abs' x e₁) e₂)) (subst (maxBeta e₂) (bind x (maxBeta e₁))) := .β (MaxBeta_maxBeta _) (MaxBeta_maxBeta _)
+      cases her.deterministic this
+      exact .β (.ofAbs ih₁) ih₂
+    | .β .. | .var | .app .. => unfold maxBeta; exact .app ih₁ ih₂
 
-theorem diamond (h₁ : e ▷β e₁) (h₂ : e ▷β e₂) : ∃ e', e₁ ▷β e' ∧ e₂ ▷β e' :=
-  ⟨maxBeta e, maxBeta.max h₁, maxBeta.max h₂⟩
-
-theorem diamond' (h₁ : e ▷β* e₁) (h₂ : e ▷β* e₂) : ∃ e', e₁ ▷β* e' ∧ e₂ ▷β* e' := by
-  induction h₁ generalizing e₂ with
-  | base h₁ =>
-    rename_i e₁
-    suffices ∃ e', e₁ ▷β* e' ∧ e₂ ▷β e' from
-      let ⟨e', he, he'⟩ := this
-      ⟨e', he, .base he'⟩
-    induction h₂ generalizing e₁ with
-    | base h₂ =>
-      let ⟨e₁, he₁, he₁'⟩ := diamond h₁ h₂
-      exact ⟨_, .base he₁, he₁'⟩
-    | refl => exact ⟨_, .refl, h₁⟩
-    | trans _ _ diamond'_h₂ diamond'_h₂' =>
-      let ⟨e₁, he₁, he₁'⟩ := diamond'_h₂ h₁
-      let ⟨e₂, he₂, he₂'⟩ := diamond'_h₂' he₁'
-      exact ⟨e₂, .trans he₁ he₂, he₂'⟩
-  | refl => exact ⟨e₂, h₂, .refl⟩
-  | trans _ _ diamond'_h₁ diamond'_h₁' =>
-    let ⟨e₁, he₁, he₁'⟩ := diamond'_h₁ h₂
-    let ⟨e₂, he₂, he₂'⟩ := diamond'_h₁' he₁
-    exact ⟨e₂, he₂, .trans he₁' he₂'⟩
+theorem diamond : Diamond BetaParallel := λ h₁ h₂ =>
+  ⟨maxBeta _, maxBeta.max h₁, maxBeta.max h₂⟩
 
 theorem betaConfluence (h₁ : e ↠β e₁) (h₂ : e ↠β e₂) : ∃ e', e₁ ↠β e' ∧ e₂ ↠β e' :=
-  let ⟨e', h₁', h₂'⟩ := BetaParallel.diamond' (BetaParallel.clos₁ h₁) (BetaParallel.clos₁ h₂)
-  ⟨e', BetaParallel.clos₂ h₁', BetaParallel.clos₂ h₂'⟩
+  let ⟨e', h₁', h₂'⟩ := ReflexiveTransitiveClosure.diamond diamond (BetaParallel.multiOfBetaReduction h₁) (BetaParallel.multiOfBetaReduction h₂)
+  ⟨e', BetaParallel.multiToBetaReduction h₁', BetaParallel.multiToBetaReduction h₂'⟩
 
 end Confluence
 
