CoNat.lean
@@ -1,0 +1,136 @@
+def CoNat := { f : Nat → Bool // ∀ i, f i || !f i.succ }
+--def CoNat := { f : Nat → Bool // ∀ i, f i.succ → f i }
+
+def CoNat.ofNat (n : Nat) : CoNat :=
+  ⟨(Nat.blt · n), λ _ => by simp [← Bool.not_eq_true]; exact if h : _ then .inl h else .inr (h ∘ Nat.lt_of_succ_lt)⟩
+
+def CoNat.inf : CoNat :=
+  ⟨λ _ => true, λ _ => rfl⟩
+
+theorem lemma32 {x : CoNat} (h : x.val n = false) : ∃ k, k ≤ n ∧ x = .ofNat k :=
+  lemma32 n.zero_le λ _ hj => nomatch hj
+where
+  lemma32 {k} (hk : k ≤ n) (hx : ∀ i, i < k → x.val i) : ∃ k, k ≤ n ∧ x = .ofNat k := by
+    generalize hm : n - k = m
+    induction m generalizing k with
+    | zero =>
+      cases k.zero_add ▸ Nat.eq_add_of_sub_eq hk hm
+      exact ⟨n, .refl, Subtype.eq <| funext λ i => .symm <| if hi : i < n then by simp [CoNat.ofNat, hi, hx] else by
+        apply Eq.trans (b := false)
+        . simp [CoNat.ofNat, ← Bool.not_eq_true, hi]
+        . apply Eq.symm
+          have := Nat.ge_of_not_lt hi
+          clear hi
+          induction this with
+          | refl => exact h
+          | step _ ih =>
+            have := x.property ‹_›
+            simp [ih] at this
+            exact this
+      ⟩
+    | succ m ih =>
+      cases hx' : x.val k with
+      | false =>
+        exact ⟨k, hk, Subtype.eq <| funext λ i => .symm <| if hi : i < k then by simp [CoNat.ofNat, hi, hx] else by
+          apply Eq.trans (b := false)
+          . simp [CoNat.ofNat, ← Bool.not_eq_true, hi]
+          . apply Eq.symm
+            have := Nat.ge_of_not_lt hi
+            clear hi
+            induction this with
+            | refl => exact hx'
+            | step _ ih =>
+              have := x.property ‹_›
+              simp [ih] at this
+              exact this
+        ⟩
+      | true =>
+        apply ih (k := k.succ)
+        . apply Nat.lt_of_le_of_ne hk
+          intro h
+          cases h
+          cases h.symm.trans hx'
+        . intro i hi
+          cases hi with
+          | refl => exact hx'
+          | step hi => apply hx; exact hi
+        . apply Nat.sub_eq_of_eq_add
+          exact Nat.eq_add_of_sub_eq hk hm |>.trans <| m.succ_add k
+
+theorem lemma33 {x : CoNat} (hx : ∀ n, x ≠ .ofNat n) : x = .inf :=
+  Subtype.eq <| funext λ i =>
+    match h : x.val i with
+    | true => rfl
+    | false => have ⟨k, _, hk⟩ := lemma32 h; nomatch hx k hk
+
+theorem lemma34 (x : CoNat) : ¬(x ≠ .inf ∧ ∀ n, x ≠ .ofNat n) :=
+  λ h => h.left <| lemma33 h.right
+
+theorem Nat.blt_irrefl : blt n n = false := by
+  simp [← Bool.not_eq_true]
+
+theorem Nat.blt_succ_self : blt n n.succ = true := by
+  simp [Nat.lt_succ_self]
+
+section
+
+variable (p : CoNat → Bool)
+
+def CoNat.find' : Nat → Bool
+  | .zero => p (.ofNat .zero)
+  | .succ i => find' i && p (.ofNat i.succ)
+
+def CoNat.find : CoNat :=
+  ⟨find' p, λ i => by dsimp [find']; cases find' .. <;> rfl⟩
+
+theorem CoNat.find_ (p : CoNat → Bool) (h : p (find p)) : ∀ x, p x := by
+  have h₁ : ∀ n, find p ≠ .ofNat n := by
+    intro n hn
+    rw [hn] at h
+    have : find' p n = Nat.blt n n := congrFun (congrArg Subtype.val hn) n
+    rw [Nat.blt_irrefl] at this
+    cases n with
+    | zero => cases h.symm.trans this
+    | succ n =>
+      dsimp only [find'] at this
+      simp [← Bool.not_eq_true] at this
+      apply this
+      have := congrFun (congrArg Subtype.val hn) n
+      simp [find, ofNat, Nat.blt_succ_self] at this
+      exact ⟨this, h⟩
+  have h₂ : find p = .inf := lemma33 h₁
+  have h₃ : ∀ n, p (.ofNat n) := λ n =>
+    have : find' p n := congrFun (congrArg Subtype.val h₂) n
+    match n with
+    | .zero => this
+    | .succ n => by simp [find'] at this; exact this.right
+  intro x
+  cases hx : p x with
+  | true => rfl
+  | false =>
+    apply False.elim
+    apply lemma34 x ⟨_, _⟩
+    . intro h
+      cases h
+      cases hx.symm.trans <| h₂ ▸ h
+    . intro n h
+      cases h
+      cases hx.symm.trans <| h₃ n
+
+def CoNat.forall : Bool :=
+  p <| find p
+
+end
+
+instance [BEq α] : BEq (CoNat → α) where
+  beq f g := CoNat.forall λ x => f x == g x
+
+instance [BEq α] [LawfulBEq α] : LawfulBEq (CoNat → α) where
+  eq_of_beq {f g} h := funext (LawfulBEq.eq_of_beq <| CoNat.find_ (λ x => f x == g x) h ·)
+  rfl := LawfulBEq.rfl (α := α)
+
+instance [BEq α] [LawfulBEq α] : DecidableEq α
+  | a, b =>
+    match h : a == b with
+    | true => isTrue <| eq_of_beq h
+    | false => isFalse (nomatch show _ = true from h.symm.trans <| · ▸ LawfulBEq.rfl)
