Common/Util.lean
@@ -1,0 +1,26 @@
+def Var := Nat deriving DecidableEq
+
+namespace Var
+
+protected def toString (x : Var) : String :=
+  ⟨toString x []⟩
+where
+  toString x l :=
+    let l := Char.ofNat ('a'.toNat + x % 26) :: l
+    match h : x / 26 with
+    | 0 => l
+    | q + 1 =>
+      have := h ▸ Nat.div_le_self ..
+      toString q l
+
+instance instToString : ToString Var := ⟨Var.toString⟩
+
+instance instOfNat : OfNat Var n := ⟨n⟩
+
+def ofString : String → Var
+  | ⟨l⟩ =>
+    l.foldl (λ x c => (x + 1) * 26 + (c.toNat - 'a'.toNat) % 26) 0 - 26 ^ l.length
+
+instance instCoeString : Coe String Var := ⟨ofString⟩
+
+end Var
