CurryParadox.lean
@@ -1,0 +1,12 @@
+unsafe inductive Curry (α : Sort u)
+  | mk : (Curry α → α) → Curry α
+
+noncomputable section
+
+unsafe def Curry.get {α : Sort u} (c : Curry α) : α :=
+  rec (· c) c
+
+unsafe def inhabit {α : Sort u} : α :=
+  Curry.get ⟨Curry.get⟩
+
+end
