Ind.lean
@@ -1,0 +1,435 @@
+import Mathlib.Data.Nat.Basic
+
+syntax (name := coinductive) "coinductive " declId bracketedBinder* (" : " term)? (ppLine "| " ident " : " term)* : command
+
+open Lean
+
+abbrev CommandMacroM := StateT (Array Command) MacroM
+
+def CommandMacroM.push (c : CommandMacroM Command) : CommandMacroM Unit :=
+  do modify (·.push (← c))
+
+def CommandMacroM.run (x : CommandMacroM Unit) : MacroM Command := do
+  let (_, cs) ← x #[]
+  return ⟨mkNullNode cs⟩
+
+partial def splitArrows (t : Term) (args : Array Term := #[]) : Array Term × Term :=
+  match t with
+  | `($arg → $ret) => splitArrows ret (args.push arg)
+  | _ => (args, t)
+
+partial def joinArrows : List Term → Term → MacroM Term
+  | [], r => return r
+  | l :: ls, r => do `($l → $(← joinArrows ls r))
+
+partial def appHead : Term → Term
+  | `($fn $_) => appHead fn
+  | t => t
+
+structure CtorView where
+  id : Ident
+  argTypes : Array (Term × Bool)
+  retType : Term
+
+structure CoInductiveView where
+  id : Ident
+  levels : Array Ident
+  binders : TSyntaxArray ``Parser.Term.bracketedBinder
+  params : Array Ident
+  type : Term
+  ctors : Array CtorView
+
+def CoInductiveView.ofSyntax : Syntax → MacroM CoInductiveView
+  | `(coinductive $id$[.{$levels?,*}]? $binders* $[: $type?]? $[| $ids : $types]*) => do
+    let params := binders.map Elab.Command.getBracketedBinderIds |>.flatten.map mkIdent
+    let ty ← `(@$id $params*)
+    return {
+      id
+      levels := match levels? with | some levels => levels.getElems | none => #[]
+      binders
+      params
+      type := type?.getD <| ← `(Type _)
+      ctors := ids.zipWith types λ ctorId type =>
+        let (argTypes, _) := splitArrows type
+        let argTypes := argTypes.map λ argType =>
+          if (appHead argType).raw.matchesIdent id.getId
+          then (ty, true)
+          else (argType, false)
+        { id := ctorId, argTypes, retType := ty }
+    }
+  | _ => Macro.throwUnsupported
+
+@[macro «coinductive»]
+def expandCoInductive : Macro := λ stx => CommandMacroM.run do
+  let view ← CoInductiveView.ofSyntax stx
+  let ctors := view.ctors.map (·.id)
+
+  let Approx := mkIdent <| view.id.getId ++ `Approx
+  let «⋯» := mkIdent `«⋯»
+  let types ← view.ctors.mapM λ ctor => do
+    let args ← ctor.argTypes.mapM λ
+      | (arg, false) => return arg
+      | (_, true) => `(@$Approx $view.params* ℓ)
+    joinArrows args.toList (← `(@$Approx $view.params* (.succ ℓ)))
+  CommandMacroM.push `(
+    inductive $Approx.{$view.levels,*} $view.binders* : Nat → $view.type
+      | $«⋯»:ident : @$Approx $view.params* .zero
+    $[| $ctors:ident {ℓ} : $types]*
+  )
+
+  let Agree := mkIdent <| view.id.getId ++ `Agree
+  let (binders, types) := Array.unzip <| ← view.ctors.mapM λ ctor => do
+    let (binders, args) := Array.unzip <| ← ctor.argTypes.mapM λ
+      | (_, false) => do
+        let x := mkIdent <| ← Elab.Term.mkFreshBinderName
+        return (#[x], #[], x, x)
+      | (_, true) => do
+        let x₁ := mkIdent <| ← Elab.Term.mkFreshBinderName
+        let x₂ := mkIdent <| ← Elab.Term.mkFreshBinderName
+        return (#[x₁, x₂], #[← `($Agree $x₁ $x₂)], x₁, x₂)
+    let (ihs, args) := args.unzip
+    let (args₁, args₂) := args.unzip
+    return (binders.flatten, ← joinArrows ihs.flatten.toList <| ← `($Agree (.$ctor.id $args₁*) (.$ctor.id $args₂*)))
+  CommandMacroM.push `(
+    inductive $Agree {$view.params*} : ∀ {ℓ₁ ℓ₂}, @$Approx $view.params* ℓ₁ → @$Approx $view.params* ℓ₂ → Prop
+      | $«⋯»:ident {x} : $Agree .«⋯» x
+    $[| $ctors:ident {$binders*} : $types]*
+  )
+
+  let Pattern := mkIdent <| view.id.getId ++ `Pattern
+  let types ← view.ctors.mapM λ ctor => do
+    let args ← ctor.argTypes.mapM λ
+      | (arg, false) => return arg
+      | (_, true) => `(α)
+    joinArrows args.toList (← `(@$Pattern $view.params* α))
+  CommandMacroM.push `(
+    inductive $Pattern.{u, $view.levels,*} $view.binders* (α : Type u)
+    $[| $ctors:ident : $types]*
+  )
+
+  let map := mkIdent <| Pattern.getId ++ `map
+  let mapApprox := mkIdent <| Pattern.getId ++ `mapApprox
+  let mapAgree := mkIdent <| Pattern.getId ++ `mapAgree
+  let (binders, args) := Array.unzip <| ← view.ctors.mapM λ ctor => do
+    let (binders, args) := Array.unzip <| ← ctor.argTypes.mapM λ
+      | (_, false) => do
+        let x := mkIdent <| ← Elab.Term.mkFreshBinderName
+        return (x, x, #[])
+      | (_, true) => do
+        let x := mkIdent <| ← Elab.Term.mkFreshBinderName
+        return (x, ← `(f $x), #[← `(h $x)])
+    let (args₁, args₂) := args.unzip
+    return (← `($ctor.id $binders*), ← `(.$ctor.id $args₁*), ← `(.$ctor.id $args₂.flatten*))
+  let (args₁, args₂) := args.unzip
+  CommandMacroM.push `(
+    @[simp]
+    def $map {$view.params* α β} (f : α → β) : @$Pattern $view.params* α → @$Pattern $view.params* β
+    $[| $binders => $args₁]*
+    @[simp]
+    def $mapApprox {$view.params* α ℓ} (f : α → @$Approx $view.params* ℓ) : @$Pattern $view.params* α → @$Approx $view.params* ℓ.succ
+    $[| $binders => $args₁]*
+    theorem $mapAgree {$view.params* α ℓ₁ ℓ₂} {f : α → @$Approx $view.params* ℓ₁} {g : α → @$Approx $view.params* ℓ₂} {x} (h : ∀ x, $Agree (f x) (g x)) : $Agree ($mapApprox f x) ($mapApprox g x) :=
+      match x with
+      $[| $binders => $args₂]*
+  )
+
+  let corec := mkIdent <| view.id.getId ++ `corec
+  CommandMacroM.push `(
+    def $view.id.{$view.levels,*} $view.binders* := { f : ∀ ℓ, @$Approx $view.params* ℓ // ∀ ℓ, $Agree (f ℓ) (f ℓ.succ) }
+    def $corec {$view.params* α} (f : α → @$Pattern $view.params* α) (x : α) : @$view.id $view.params* where
+      val ℓ := ℓ.rec (λ _ => .«⋯») (λ _ ih x => $mapApprox ih (f x)) x
+      property ℓ := ℓ.rec (λ _ => .«⋯») (λ _ ih _ => $mapAgree ih) x
+  )
+
+  let wrappers ← CommandMacroM.run do
+    for ctor in view.ctors do
+      let (binders, args) := Array.unzip <| ← ctor.argTypes.mapM λ
+        | (_, false) => do
+          let x := mkIdent <| ← Elab.Term.mkFreshBinderName
+          return (x, x, #[])
+        | (_, true) => do
+          let x := mkIdent <| ← Elab.Term.mkFreshBinderName
+          return (x, ← `($(x).val ℓ), #[← `($(x).property ℓ)])
+      let (args₁, args₂) := args.unzip
+      let type ← joinArrows (ctor.argTypes.map (·.fst)).toList ctor.retType
+      CommandMacroM.push `(
+        def $ctor.id {$view.params*} : $type := λ $binders* => {
+          val := λ | .zero => .«⋯» | .succ ℓ => .$ctor.id $args₁*
+          property := λ | .zero => .«⋯» | .succ ℓ => .$ctor.id $args₂.flatten*
+        }
+      )
+  CommandMacroM.push `(
+    namespace $view.id
+    $wrappers
+    end $view.id
+  )
+
+  let refl := mkIdent <| Agree.getId ++ `refl
+  let (binders, args) := Array.unzip <| ← view.ctors.mapM λ ctor => do
+    let (binders, args) := Array.unzip <| ← ctor.argTypes.mapM λ
+      | (_, false) => do
+        let x := mkIdent <| ← Elab.Term.mkFreshBinderName
+        return (x, #[])
+      | (_, true) => do
+        let x := mkIdent <| ← Elab.Term.mkFreshBinderName
+        return (x, #[← `($refl)])
+    return (← `(.$ctor.id $binders*), ← `(.$ctor.id $args.flatten*))
+  CommandMacroM.push `(
+    theorem $refl {$view.params* ℓ} : ∀ {x : @$Approx $view.params* ℓ}, $Agree x x
+      | .«⋯» => .«⋯»
+      $[| $binders => $args]*
+  )
+
+  let trans := mkIdent <| Agree.getId ++ `trans
+  let (binders₁, args) := Array.unzip <| ← view.ctors.mapM λ ctor => do
+    let (binders₁, args) := Array.unzip <| ← ctor.argTypes.mapM λ
+      | (_, false) => return (#[], #[], #[])
+      | (_, true) => do
+        let x₁ := mkIdent <| ← Elab.Term.mkFreshBinderName
+        let x₂ := mkIdent <| ← Elab.Term.mkFreshBinderName
+        return (#[x₁], #[x₂], #[← `($trans $x₁ $x₂)])
+    let (binders₂, args) := args.unzip
+    return (← `(.$ctor.id $binders₁.flatten*), ← `(.$ctor.id $binders₂.flatten*), ← `(.$ctor.id $args.flatten*))
+  let (binders₂, args) := args.unzip
+  CommandMacroM.push `(
+    theorem $trans {$view.params* ℓ ℓ'} {x₁ : @$Approx $view.params* ℓ} {x₂ : @$Approx $view.params* ℓ.succ} {x₃ : @$Approx $view.params* ℓ'} : $Agree x₁ x₂ → $Agree x₂ x₃ → $Agree x₁ x₃
+      | .«⋯», _ => .«⋯»
+    $[| $binders₁, $binders₂ => $args]*
+  )
+
+  let property := mkIdent <| view.id.getId ++ `property
+  CommandMacroM.push `(
+    theorem $property {$view.params*} (x : @$view.id $view.params*) ⦃ℓ₁ ℓ₂⦄ (h : ℓ₁ ≤ ℓ₂) : $Agree (x.val ℓ₁) (x.val ℓ₂) := by
+      have ⟨ℓ, h⟩ := Nat.exists_eq_add_of_le h
+      cases h
+      exact ℓ.rec (λ _ => $refl) (λ ℓ ih ℓ₁ => $trans (Subtype.property x ℓ₁) (ℓ₁.succ_add ℓ ▸ ih _ :)) ℓ₁
+  )
+
+  let cases := mkIdent <| view.id.getId ++ `cases
+  let (args, minors) := Array.unzip <| ← view.ctors.mapM λ ctor => do
+    let args ← ctor.argTypes.mapM λ _ => return mkIdent <| ← Elab.Term.mkFreshBinderName
+    return (args, ← `(Parser.Term.bracketedBinderF| ($ctor.id : ∀ $args:ident*, motive ($ctor.id $args*))))
+  let arms ← (view.ctors.zip args).mapIdxM λ i (ctor, args) => do
+    let otherCtors := ctors.eraseIdx i
+    let rhs ←
+      `(have : x = .$ctor.id $args* := Subtype.eq <| funext λ
+          | .zero => match x.val .zero with | .«⋯» => rfl
+          | .succ ℓ =>
+            have := h ▸ $property x ℓ.zero_lt_succ
+            match h' : x.val ℓ.succ with
+          $[| .$otherCtors .. => by cases h' ▸ this]*
+            | .$ctor.id .. => by
+              cases h' ▸ this
+              congr
+              all_goals
+                dsimp only []
+                split <;> rename_i h'' <;> cases h' ▸ h''
+                rfl
+        this ▸ $ctor.id $args*)
+    let ihs := args.zip ctor.argTypes |>.filterMap λ | (_, _, false) => none | (arg, _, true) => some arg
+    ihs.foldrM (init := rhs) λ arg rhs =>
+      `(let $arg := {
+          val := λ ℓ =>
+            match h' : x.val ℓ.succ with
+          $[| .$otherCtors .. => nomatch (h' ▸ h ▸ x.property ℓ.zero_lt_succ :)]*
+            | .$ctor.id $args* => $arg
+          property := λ ℓ =>
+            match h₁ : x.val ℓ.succ with
+          $[| .$otherCtors .. => nomatch (h₁ ▸ h ▸ x.property ℓ.zero_lt_succ :)]*
+            | .$ctor.id .. =>
+              match h₂ : x.val ℓ.succ.succ with
+            $[| .$otherCtors .. => nomatch (h₂ ▸ h ▸ x.property ℓ.succ.zero_lt_succ :)]*
+              | .$ctor.id .. => by
+                dsimp only []
+                split <;> rename_i h₁' <;> cases h₁ ▸ h₁'
+                split <;> rename_i h₂' <;> cases h₂ ▸ h₂'
+                match h₁ ▸ h₂ ▸ x.property ℓ.succ.le_succ with
+                | .$ctor.id $ihs:ident* => exact $arg
+        }
+        $rhs)
+  CommandMacroM.push `(
+    @[elab_as_elim]
+    def $cases.{u} {$view.params*} {motive : @$view.id $view.params* → Sort u} $minors* x : motive x :=
+      match h : x.val (.succ .zero) with
+      $[| .$ctors $args* => $arms]*
+  )
+
+  let unfold := mkIdent <| view.id.getId ++ `unfold
+  CommandMacroM.push `(
+    def $unfold {$view.params*} : @$view.id $view.params* → @$Pattern $view.params* (@$view.id $view.params*) :=
+      $cases $(← ctors.mapM λ ctor => `(.$ctor))*
+  )
+
+coinductive CoNat
+  | zero : CoNat
+  | succ : CoNat → CoNat
+
+coinductive CoList (α : Type u)
+  | nil : CoList
+  | cons : α → CoList → CoList
+
+@[simp]
+theorem CoNat.cases_zero zero succ : @cases motive zero succ .zero = zero := rfl
+
+@[simp]
+theorem CoNat.cases_succ zero succ n : @cases motive zero succ (.succ n) = succ n := rfl
+
+@[simp]
+theorem CoNat.unfold_zero : unfold zero = .zero := rfl
+
+@[simp]
+theorem CoNat.unfold_succ n : unfold (succ n) = .succ n := rfl
+
+@[simp]
+theorem CoList.cases_nil nil cons : @cases α motive nil cons .nil = nil := rfl
+
+@[simp]
+theorem CoList.cases_cons nil cons x xs : @cases α motive nil cons (.cons x xs) = cons x xs := rfl
+
+@[simp]
+theorem CoList.unfold_nil : @unfold α nil = .nil := rfl
+
+@[simp]
+theorem CoList.unfold_cons x xs : @unfold α (cons x xs) = .cons x xs := rfl
+
+@[simp]
+theorem CoNat.unfold_corec f x : unfold (@corec α f x) = (f x).map (corec f) := by
+  unfold Pattern.map
+  split <;> rename_i h
+    <;> simp [unfold, cases, corec]
+    <;> split <;> rename_i h' <;> cases h ▸ h'
+    <;> congr
+  funext ℓ
+  split <;> rename_i h' <;> cases h ▸ h'
+  rfl
+
+@[simp]
+theorem CoList.unfold_corec : unfold (corec f x) = (f x).map (corec f) := by
+  unfold Pattern.map
+  split <;> rename_i h
+    <;> simp [unfold, cases, corec]
+    <;> split <;> rename_i h' <;> cases h ▸ h'
+    <;> congr
+  funext ℓ
+  split <;> rename_i h' <;> cases h ▸ h'
+  rfl
+
+theorem dcongrArg.{u, v} {α : Sort u} {β : α → Sort v} {a₁ a₂ : α} (f : ∀ x, β x) (h : a₁ = a₂) : HEq (f a₁) (f a₂) :=
+  by cases h; rfl
+
+theorem CoNat.cases_corec zero succ f x : @cases motive zero succ (@corec α f x) = match h : f x with | .zero => (Subtype.eq <| funext λ | .zero => rfl | .succ ℓ => by simp [corec, h, CoNat.zero] : corec f x = .zero) ▸ zero | .succ x' => (Subtype.eq <| funext λ | .zero => rfl | .succ ℓ => by simp [corec, h, CoNat.succ]: corec f x = .succ (corec f x')) ▸ succ (corec f x') := by
+  split
+    <;> rename_i h
+    <;> simp [cases, corec]
+    <;> split <;> rename_i h' <;> cases h ▸ h'
+  . rfl
+  . rename_i x'
+    generalize hA : succ _ = A
+    generalize hB : succ _ = B
+    sorry
+
+def CoNat.ofNat₁ : Nat → CoNat
+  | .zero => .zero
+  | .succ n => .succ (ofNat₁ n)
+
+def CoNat.ofNat₂ : Nat → CoNat :=
+  corec λ | .zero => .zero | .succ n => .succ n
+
+theorem CoNat.ofNat₁_eq_ofNat₂ : ofNat₁ n = ofNat₂ n := by
+  apply Subtype.eq
+  funext ℓ
+  induction n generalizing ℓ with
+  | zero => cases ℓ <;> rfl
+  | succ d ih =>
+    cases ℓ with
+    | zero => rfl
+    | succ ℓ => exact congrArg _ <| ih ℓ
+
+def CoNat.add (a b : CoNat) : CoNat :=
+  corec (λ (a, b) =>
+    match b.unfold with
+    | .zero =>
+      match a.unfold with
+      | .zero => .zero
+      | .succ a => .succ (a, b)
+    | .succ b => .succ (a, b)
+  ) (a, b)
+
+theorem CoNat.add_zero : add a zero = a := by
+  apply Subtype.eq
+  funext ℓ
+  dsimp [add, corec]
+  induction ℓ with
+  | zero => cases a.val .zero; rfl
+  | succ ℓ ih =>
+    dsimp [add, corec, zero, succ]
+    sorry
+
+def CoNat.toNat : Nat → CoNat → Option Nat
+  | .zero, _ => none
+  | .succ m, n =>
+    match n.unfold with
+    | .zero => some .zero
+    | .succ n => n.toNat m |>.map .succ
+
+theorem CoNat.add_ofNat₁ : add (ofNat₁ a) (ofNat₁ b) = ofNat₁ (a + b) := by
+  apply Subtype.eq
+  funext ℓ
+  induction b generalizing ℓ with
+  | zero =>
+    dsimp only [ofNat₁, ofNat₂, corec, zero, succ, add]
+    dsimp
+    induction ℓ with
+    | zero =>
+      dsimp
+      sorry
+    | succ ℓ ih =>
+      sorry
+  | succ b ih =>
+    sorry
+
+theorem CoNat.add_ofNat₂ : add (ofNat₂ a) (ofNat₂ b) = ofNat₂ (a + b) := by
+  apply Subtype.eq
+  funext ℓ
+  induction b generalizing ℓ with
+  | zero =>
+    dsimp only [ofNat₁, ofNat₂, corec, zero, succ, add]
+    dsimp
+    induction ℓ with
+    | zero => rfl
+    | succ ℓ ih =>
+      dsimp
+      sorry
+  | succ b ih =>
+    sorry
+  sorry
+
+/-
+inductive CoNat'
+  | zero : CoNat'
+  | succ' : Thunk CoNat' → CoNat'
+  deriving Inhabited
+
+def CoNat'.succ (n : CoNat') : CoNat' :=
+  succ' n
+
+def CoNat'.cases {motive : CoNat' → Sort u} (zero : motive zero) (succ : ∀ n, motive (succ n)) n : motive n :=
+  match n with
+  | .zero => zero
+  | .succ' n => succ n.get
+
+partial def CoNat'.corec (f : α → Option α) (x : α) : CoNat' :=
+  match f x with
+  | none => zero
+  | some x => succ' (corec f x)
+
+structure Hide (α : Type u) where
+  x : α
+
+instance : Repr (Hide α) where
+  reprPrec _ _ := "⟨hidden⟩"
+
+#eval 2 + 2
+#eval Hide.mk (CoNat'.corec some ())
+#eval 2 + 2
+-/
