Param.lean
@@ -1,0 +1,77 @@
+@[simp]
+theorem List.map_append : map f (l ++ l') = map f l ++ map f l' := by
+  induction l with
+  | nil => rfl
+  | cons => dsimp!; congr
+
+namespace Param
+
+class Functor (f : Sort u → Sort v) where
+  map : (α → β) → f α → f β
+  map_id (x : f α) : map id x = x
+  map_comp (g : β → γ) (h : α → β) (x : f α) : map (g ∘ h) x = map g (map h x)
+
+class ContraFunctor (f : Sort u → Sort v) where
+  map : (α → β) → f β → f α
+  map_id (x : f α) : map id x = x
+  map_comp (g : β → γ) (h : α → β) (x : f γ) : map (g ∘ h) x = map h (map g x)
+
+instance : Functor List where
+  map := List.map
+  map_id x := by
+    induction x with
+    | nil => rfl
+    | cons => dsimp!; congr
+  map_comp _ _ x := by
+    induction x with
+    | nil => rfl
+    | cons => dsimp!; congr
+
+def Set (α : Sort u) := α → Prop
+
+instance : Functor Set where
+  map f s y := ∃ x, s x ∧ f x = y
+  map_id _ := funext λ _ => propext ⟨λ ⟨_, p, rfl⟩ => p, λ p => ⟨_, p, rfl⟩⟩
+  map_comp _ _ _ := funext λ _ => propext ⟨λ ⟨x, p, h⟩ => ⟨_, ⟨x, p, rfl⟩, h⟩, λ ⟨_, ⟨x, p, rfl⟩, h⟩ => ⟨x, p, h⟩⟩
+
+instance : ContraFunctor Set where
+  map f s x := s (f x)
+  map_id _ := rfl
+  map_comp _ _ _ := rfl
+
+inductive List.lift (r : α → β → Prop) : List α → List β → Prop
+  | nil : lift r [] []
+  | cons : r x x' → lift r l l' → lift r (x :: l) (x' :: l')
+
+theorem List.lift_fun_eq_map : lift (g · = ·) l l' ↔ List.map g l = l' := by
+  induction l generalizing l' with
+  | nil => cases l'; exact ⟨λ _ => rfl, λ _ => .nil⟩; exact ⟨λ h => nomatch h, λ h => nomatch h⟩
+  | cons _ _ ih => cases l'; exact ⟨λ h => nomatch h, λ h => nomatch h⟩; exact ⟨λ | .cons rfl h => congrArg (List.cons _) <| ih.mp h, λ h => have ⟨h₁, h₂⟩ := List.cons.inj h; .cons h₁ <| ih.mpr h₂⟩
+
+def ft₁ (f : ∀ {α}, List α → List α) := ∀ {α β} (r : α → β → Prop) {l l'} (h : List.lift r l l'), List.lift r (f l) (f l')
+def ft₁' (f : ∀ {α}, List α → List α) := ∀ {α β} (g : α → β) (l : List α), (f l).map g = f (l.map g)
+
+example : ft₁ f → ft₁' f
+  | h, _, _, _, _ => List.lift_fun_eq_map.mp <| h _ <| List.lift_fun_eq_map.mpr rfl
+
+/-
+ forall (x, y) in lift{[]}(R). (f x, f y) in lift{[]}(R)
+
+lift{[]}(R)
+  = {([], [])}
+  u {(x : xs, y : ys) | ((x, y) in R) && ((xs, ys) in lift{[]}(R))}
+-/
+
+example : List.reverse (Functor.map f x) = Functor.map f (List.reverse x) := by
+  dsimp [Functor.map]
+  induction x with
+  | nil => rfl
+  | cons => simp! [*]
+
+def Set.comp (s : Set α) : Set α
+  | x => !s x
+
+example : Set.comp (ContraFunctor.map f s) = ContraFunctor.map f (Set.comp s) := rfl
+
+def List.toSet [BEq α] (l : List α) : Set α
+  | x => l.contains x
