Sort1.lean
@@ -1,0 +1,228 @@
+class Preorder (α) extends LE α where
+  trans {x y z : α} : x ≤ y → y ≤ z → x ≤ z
+  refl (x : α) : x ≤ x
+
+class TotalPreorder (α) extends Preorder α where
+  total (x y : α) : x ≤ y ∨ y ≤ x
+  refl x := (total x x).elim id id
+
+theorem le_of_not_le [I : TotalPreorder α] {x y : α} (h : ¬x ≤ y) : y ≤ x :=
+  (I.total x y).elim (False.elim ∘ h) id
+
+instance : TotalPreorder Nat where
+  trans := Nat.le_trans
+  total := Nat.le_total
+
+inductive List.Chain (R : α → α → Prop) : α → List α → Prop
+  | nil : Chain R a []
+  | cons : R a b → Chain R b l → Chain R a (b :: l)
+
+def List.Chain' (R : α → α → Prop) : List α → Prop
+  | [] => True
+  | a :: l => Chain R a l
+
+inductive List.Perm : List α → List α → Prop
+  | nil : Perm [] []
+  | cons (x) : Perm l₁ l₂ → Perm (x :: l₁) (x :: l₂)
+  | swap (x y l) : Perm (y :: x :: l) (x :: y :: l)
+  | trans : Perm l₁ l₂ → Perm l₂ l₃ → Perm l₁ l₃
+
+@[simp]
+theorem List.Perm.refl : (l : List α) → Perm l l
+  | [] => nil
+  | x :: l => cons x (refl l)
+
+theorem List.Perm.symm (h : Perm l₂ l₁) : Perm l₁ l₂ := by
+  induction h with
+  | nil => exact nil
+  | cons x _ ih => exact cons x ih
+  | swap x y l => exact swap y x l
+  | trans _ _ ih₁ ih₂ => exact trans ih₂ ih₁
+
+theorem List.Perm.swap' (y) (h : Perm l₁ (x :: l₂)) : Perm (y :: l₁) (x :: y :: l₂) :=
+  trans (cons y h) (swap x y l₂)
+
+theorem List.Perm.length_eq (h : Perm l₁ l₂) : length l₁ = length l₂ := by
+  induction h <;> simp [*]
+
+theorem List.Perm.middle (x : α) : ∀ l₁ l₂, Perm (l₁ ++ x :: l₂) (x :: l₁ ++ l₂)
+  | [], _ => refl _
+  | y :: l₁, l₂ => swap' y (middle x l₁ l₂)
+
+theorem List.Perm.inv : Perm (l₁ ++ x :: r₁) (l₂ ++ x :: r₂) → Perm (l₁ ++ r₁) (l₂ ++ r₂) := by
+  generalize h₁ : l₁ ++ x :: r₁ = s₁
+  generalize h₂ : l₂ ++ x :: r₂ = s₂
+  intro h
+  induction h generalizing l₁ r₁ l₂ r₂ with
+  | nil => sorry
+  | cons y h ih =>
+    cases l₁ <;> cases l₂ <;> cases h₁ <;> cases h₂
+    . exact h
+    . exact trans h (middle _ _ _)
+    . exact trans (symm (middle _ _ _)) h
+    . exact cons y (ih rfl rfl)
+  | swap _ _ _ => sorry
+  | trans _ _ _ _ => sorry
+
+@[simp]
+theorem List.Perm.cons_iff : Perm (x :: l₁) (x :: l₂) ↔ Perm l₁ l₂ where
+  mp h := inv (l₁ := []) (l₂ := []) h
+  mpr := cons x
+
+@[simp]
+theorem List.Perm.cons_iff' : Perm (y₁ :: x :: l₁) (y₂ :: x :: l₂) ↔ Perm (y₁ :: l₁) (y₂ :: l₂) where
+  mp h := inv (l₁ := [y₁]) (l₂ := [y₂]) h
+  mpr h := trans (trans (swap x y₁ l₁) (cons x h)) (swap y₂ x l₂)
+
+@[simp]
+theorem List.Perm.swap_iff : Perm (y :: l₁) (x :: y :: l₂) ↔ Perm l₁ (x :: l₂) where
+  mp h := inv (l₁ := []) (l₂ := [x]) h
+  mpr := swap' y
+
+@[simp]
+theorem List.Perm.swap_iff' : Perm (y₁ :: x :: l₁) (x :: y₂ :: l₂) ↔ Perm (y₁ :: l₁) (y₂ :: l₂) where
+  mp h := inv (l₁ := [y₁]) (l₂ := []) h
+  mpr h := symm (swap' x (symm h))
+
+class ComparisonSort (f : ∀ {α} [I : LE α] [DecidableRel I.le], List α → List α) where
+  perm [I : LE α] [DecidableRel I.le] (l : List α) : (f l).Perm l
+  sort [I : TotalPreorder α] [DecidableRel I.le] (l : List α) : (f l).Chain' I.le
+
+section
+
+variable [I : LE α] [DecidableRel I.le]
+
+def insert (x : α) : List α → List α
+  | [] => [x]
+  | y :: l =>
+    if x ≤ y
+    then x :: y :: l
+    else y :: insert x l
+
+def insertionSort : List α → List α
+  | [] => []
+  | x :: l => insert x (insertionSort l)
+
+theorem perm_insert (x : α) (l) : (insert x l).Perm (x :: l) := by
+  induction l <;> simp [insert]; split <;> simp [*]
+
+end
+
+theorem sort_insert [I : TotalPreorder α] [DecidableRel I.le] (x) (h : l.Chain' I.le) : (insert x l).Chain' I.le := by
+  induction l
+  case nil => exact .nil
+  case cons y l ih =>
+    unfold insert
+    split
+    case _ h' => exact .cons h' h
+    case _ h' =>
+      have h' := le_of_not_le h'
+      dsimp [List.Chain']
+      cases h
+      case nil => exact .cons h' .nil
+      case cons z l h₁ h₂  =>
+        specialize ih h₁
+        unfold insert at ih ⊢
+        split
+        case _ h'' =>
+          simp [h''] at ih
+          exact .cons h' ih
+        case _ h'' =>
+          simp [h''] at ih
+          exact .cons h₂ ih
+
+instance : ComparisonSort @insertionSort where
+  perm l := by
+    induction l with
+    | nil => exact .nil
+    | cons x l ih => exact .trans (perm_insert x (insertionSort l)) (.cons x ih)
+  sort l := by
+    induction l with
+    | nil => exact trivial
+    | cons x l ih => exact sort_insert x ih
+
+section
+
+variable [I : LE α] [DecidableRel I.le]
+
+def select (x : α) : List α → α × List α
+  | [] => (x, [])
+  | y :: l =>
+    if x ≤ y
+    then ((select x l).1, y :: (select x l).2)
+    else ((select y l).1, x :: (select y l).2)
+
+theorem perm_select (x : α) (l) : ((select x l).1 :: (select x l).2).Perm (x :: l) := by
+  induction l generalizing x <;> simp [select]; split <;> simp [*]
+
+def selectionSort : List α → List α
+  | [] => []
+  | x :: l =>
+    have := Nat.le_of_eq (perm_select x l).length_eq
+    (select x l).1 :: selectionSort (select x l).2
+termination_by _ l => l.length
+
+end
+
+instance : ComparisonSort @selectionSort where
+  perm l := by
+    generalize hn : l.length = n
+    induction n generalizing l with
+    | zero =>
+      cases l with
+      | nil => exact .nil
+      | cons => cases hn
+    | succ _ ih =>
+      cases l with
+      | nil => cases hn
+      | cons x l =>
+        simp [selectionSort]
+        exact .trans (.cons _ (ih _ (Nat.succ.inj ((perm_select x l).length_eq.trans hn)))) (perm_select x l)
+  sort l := by
+    sorry
+
+-- todo: comparison in monad, time complexity
+
+section
+
+variable [Monad m] (le : α → α → m Bool)
+
+def insertM (x : α) : List α → m (List α)
+  | [] => return [x]
+  | y :: l =>
+    return if ← le x y
+      then x :: y :: l
+      else y :: (← insertM x l)
+
+def insertM' (x : α) : List α → m (List α)
+  | [] => return [x]
+  | y :: l => do
+    if ← le x y
+    then return x :: y :: l
+    else return y :: (← insertM' x l)
+
+def myLe (x y : Nat) : IO Bool := do
+  IO.println s!"{x} ≤ {y}"
+  return x ≤ y
+
+#print insertM
+#print insertM'
+
+def insertionSortM : List α → List α
+  | [] => []
+  | x :: l => insertM ifLE x (insertionSortM l)
+
+end
+
+variable [I : LE α] [DecidableRel I.le]
+
+def isLE (x y : α) (t e : List α) : List α :=
+  if x ≤ y then t else e
+
+theorem insert_eq_insertM (x : α) (l) : insert x l = insertM isLE x l := by
+  unfold isLE
+  induction l <;> simp [insert, insertM]
+  split <;> simp [*]
+
+theorem insertionSort_eq_insertionSortM (l : List α) : insertionSort l = insertionSortM isLE l := by
+  induction l <;> simp [insertionSort, insertionSortM, insert_eq_insertM, *]
