Strict.lean
@@ -1,0 +1,14 @@
+import Mathlib.Logic.Function.Basic
+
+unsafe inductive A
+  | intro : ((A → Prop) → Prop) → A
+
+unsafe def A.intro.inj : intro x = intro y → x = y :=
+  @Eq.rec A (intro x) (rec λ y _ => x = y) rfl (intro y)
+
+unsafe def f : (A → Prop) → A := (⟨Eq ·⟩)
+
+unsafe def f.inj (h : f x = f y) : x = y :=
+  congrFun (A.intro.inj h) y ▸ rfl
+
+#check Function.cantor_injective f @f.inj
